Proof of progress in... progress

theories/Functional.v
@@ -68,9 +68,9 @@ Inductive instantiation_func : ℜ -> 𝓥 -> Prop :=
 
   | itfT_init   : 
     forall (Re Re' : ℜ) (V V' : 𝓥) (τ τ' : Τ) (v : Λ),
-      Instᵣₜ(Re,V) -> newᵣᵪ(Re) ⊩ₜ τ ->
+      Instᵣₜ(Re,V) ->
       Addᵣᵪ (newᵣᵪ(Re)) (τ,τ') Re Re' -> 
-      Addᵣᵦ (newᵣᵦ(V)) ⩽ v … ⩾ V V' -> 
+      Addᵣᵦ (newᵣᵦ(V)) (⩽ v … ⩾) V V' -> 
       ∅ᵥᵪ ⋅ Re ⊫ v ∈ τ' -> 
       Instᵣₜ(Re',V')
   
@@ -81,7 +81,8 @@ Inductive instantiation_func : ℜ -> 𝓥 -> Prop :=
 
 where "'Instᵣₜ(' Re , V )" := (instantiation_func Re V).
 
-(*
+Definition all_arrow_halting := forall Re t α β,
+  ∅ᵥᵪ ⋅ Re ⊫ arr(t) ∈ (α ⟿ β ∣ ∅ᵣₛ) -> forall v, ∅ᵥᵪ ⋅ Re ⊫ v ∈ α -> halts <[t v]>.
 
 (** *** Instantiation *)
 
@@ -89,20 +90,20 @@ Lemma instantiation_is_empty_spec : forall (Re : ℜ) (V : 𝓥),
   Instᵣₜ(Re,V) -> RC.Raw.is_empty Re = RE.Raw.is_empty V.
 Proof.
   intros Re V Hinst; induction Hinst.
-  - rewrite RC.is_empty_1; auto; 
-    now rewrite RE.is_empty_1.
-  - apply RC.notEmpty_Add_spec in H0.
-    apply RE.notEmpty_Add_spec in H1.
+  - rewrite RC.OP.P.is_empty_1; auto; 
+    now rewrite RE.OP.P.is_empty_1.
+  - apply RC.notEmpty_Add_spec in H.
+    apply RE.notEmpty_Add_spec in H0.
     destruct (RC.Raw.is_empty Re') eqn:HEmp.
-    -- apply RC.is_empty_2 in HEmp; contradiction.
+    -- apply RC.OP.P.is_empty_2 in HEmp; contradiction.
     -- destruct (RE.Raw.is_empty V') eqn:HEmp'; auto.
-        apply RE.is_empty_2 in HEmp'; contradiction.
+        apply RE.OP.P.is_empty_2 in HEmp'; contradiction.
   - apply RE.notEmpty_Add_spec in H1.
     destruct (RC.Raw.is_empty Re) eqn:HEmp.
-    -- apply RC.is_empty_2 in HEmp.
+    -- apply RC.OP.P.is_empty_2 in HEmp.
         apply RC.notEmpty_find_spec in H; auto; contradiction.
     -- destruct (RE.Raw.is_empty V') eqn:HEmp'; auto.
-        apply RE.is_empty_2 in HEmp'; contradiction.
+        apply RE.OP.P.is_empty_2 in HEmp'; contradiction.
 Qed.
 
 Lemma instantiation_max : forall (Re : ℜ) (V : 𝓥),
@@ -111,22 +112,21 @@ Proof.
   intros Re V inst; induction inst.
   - rewrite RC.Ext.max_key_Empty_spec; auto.
     now rewrite RE.Ext.max_key_Empty_spec.
-  - apply RC.Ext.max_key_Add_spec in H0 as [[H0 H0'] | [H0 H0']]; auto.
-    -- rewrite H0. 
-        apply RE.Ext.max_key_Add_spec in H1 as [[H1 H1'] | [H1 H1']].
-        + rewrite H1; apply instantiation_is_empty_spec in inst as HEmp.
+  - apply RC.Ext.max_key_Add_spec in H as [[H H'] | [H H']]; auto.
+    -- rewrite H. 
+        apply RE.Ext.max_key_Add_spec in H0 as [[H0 H0'] | [H0 H0']].
+        + rewrite H0; apply instantiation_is_empty_spec in inst as HEmp.
           unfold RC.Ext.new_key,RE.Ext.new_key; rewrite HEmp.
           destruct (RE.Raw.is_empty V); auto.
-        + rewrite RE.shift_max_spec in H1'; auto.
-          assert (newᵣᵦ(V) >= maxᵣᵦ(V)). { apply RE.Ext.new_key_geq_max_key. }
+        + assert (newᵣᵦ(V) >= maxᵣᵦ(V)). { apply RE.Ext.new_key_geq_max_key. }
           lia.
-        + apply RE.shift_new_notin_spec; auto.
-    -- unfold RC.Ext.new_key in H0'. 
+        + apply RE.new_key_notin_spec; auto.
+    -- unfold RC.Ext.new_key in H'. 
         destruct (RC.Raw.is_empty Re) eqn:HEmp; try lia.
-        rewrite RC.Ext.max_key_Empty_spec in H0'; try lia.
-        now apply RC.is_empty_2.
+        rewrite RC.Ext.max_key_Empty_spec in H'; try lia.
+        now apply RC.OP.P.is_empty_2.
     -- apply RC.Ext.new_key_notin_spec; lia.
-  - unfold RE.Add in H1; rewrite H1.
+  - unfold RE.OP.P.Add in H1; rewrite H1.
     rewrite RE.Ext.max_key_add_spec_3; auto.
 Qed.
 
@@ -146,21 +146,17 @@ Proof.
   intros Re V k πτ inst; revert k πτ; induction inst; intros k' πτ' Hfin.
   - apply RC.notEmpty_find_spec in Hfin; auto; contradiction.
   - rewrite H0 in *; destruct (Resource.eq_dec (newᵣᵪ(Re)) k'); subst.
-    -- exists ([⧐ᵣₓ newᵣᵦ( V) ≤ 1] ⩽ v … ⩾); rewrite H1. 
+    -- exists (⩽ v … ⩾). 
         apply instantiation_new in inst as Hnew; rewrite Hnew.
-        now apply RE.add_eq_o.
-    -- rewrite RC.add_neq_o in Hfin; try assumption.
-        apply IHinst in Hfin as [v' Hfin]; exists ([⧐ᵣₓ (newᵣᵦ(V)) ≤ 1] v'). rewrite H1.
-        rewrite RE.add_neq_o.
-        + rewrite <- Resource.shift_valid_refl with (lb := newᵣᵦ(V)) (t := k') (k := 1).
-          ++ now apply RE.shift_find_spec.
-          ++ unfold Resource.valid; apply RE.Ext.new_key_in_spec.
-            exists v'; now apply RE.find_2.
-        + apply instantiation_new in inst; now rewrite <- inst.
+        now apply RE.OP.P.add_eq_o.
+    -- rewrite H in Hfin. rewrite RC.OP.P.add_neq_o in Hfin; try assumption.
+        apply IHinst in Hfin as [v' Hfin]; exists v'. 
+        rewrite RE.OP.P.add_neq_o; auto.
+        apply instantiation_new in inst; now rewrite <- inst.
   - destruct (Resource.eq_dec r k'); subst.
-    -- exists (⩽ … v ⩾); rewrite H1; now apply RE.add_eq_o.
+    -- exists (⩽ … v ⩾); rewrite H1; now apply RE.OP.P.add_eq_o.
     -- apply IHinst in Hfin; destruct Hfin.
-        exists x. rewrite H1; now rewrite RE.add_neq_o.
+        exists x. rewrite H1; now rewrite RE.OP.P.add_neq_o.
 Qed.
 
 #[export] 
@@ -185,96 +181,41 @@ Proof.
         + now rewrite Heq'.
 Qed.
 
-Lemma instantiation_valid : forall (Re : ℜ) V,
-  Instᵣₜ(Re,V) -> newᵣᵪ(Re) ⊩ᵣᵪ Re /\ newᵣᵦ(V) ⊩ᵣᵦ V.
-Proof.
-  intros Re V inst; induction inst.
-  - split; try now apply RC.valid_Empty_spec.
-    now apply RE.valid_Empty_spec.
-  - destruct IHinst as [IH1 IH2]; apply well_typed_implies_valid in H2 as [H2 H2']; 
-    auto; try (now apply VContext.valid_empty_spec); split.
-    -- rewrite <- RC.valid_Add_spec; eauto;
-        try (now apply RC.Ext.new_key_notin_spec; lia).
-        repeat split; simpl; unfold RC.Add in *;
-         apply RC.Ext.new_key_eq in H0 as Hnew; rewrite Hnew;
-        rewrite RC.Ext.new_key_add_new_key_spec; try lia.
-        + unfold Resource.valid; lia.
-        + apply Typ.valid_weakening with (k := newᵣᵪ( Re)); auto.
-        + apply Typ.valid_weakening with (k := newᵣᵪ( Re)); auto.
-        + apply RC.valid_weakening with (k := newᵣᵪ( Re)); auto.
-    -- rewrite <- RE.valid_Add_spec; eauto;
-        try (now apply RE.shift_new_notin_spec; eauto).
-        repeat split;
-        unfold RE.Add in *;
-        apply RE.Ext.new_key_eq in H1 as Hnew; rewrite Hnew;
-        replace (⌈ newᵣᵦ( V) ⤆ [⧐ᵣₓ newᵣᵦ( V) ≤ 1] ⩽ v … ⩾ ⌉ᵣᵦ ([⧐ᵣᵦ newᵣᵦ( V) ≤ 1] V)) 
-        with (⌈ newᵣᵦ([⧐ᵣᵦ newᵣᵦ( V) ≤ 1] V) ⤆ [⧐ᵣₓ newᵣᵦ( V) ≤ 1] ⩽ v … ⩾ ⌉ᵣᵦ 
-                    ([⧐ᵣᵦ newᵣᵦ( V) ≤ 1] V))
-        by (f_equal; rewrite RE.shift_new_spec; lia);
-        rewrite RE.Ext.new_key_add_new_key_spec; 
-        rewrite RE.shift_new_spec; auto.
-        + unfold Resource.valid; lia.
-        + replace (S (newᵣᵦ( V))) with ((newᵣᵦ( V)) + 1) by lia.
-          apply Cell.shift_preserves_valid_1.
-          unfold Cell.valid; simpl. apply instantiation_new in inst.
-          rewrite <- inst; auto.
-        + replace (S (newᵣᵦ( V))) with ((newᵣᵦ( V)) + 1) by lia.
-          now apply RE.shift_preserves_valid_1.
-  - destruct IHinst; split; auto; apply RE.Ext.new_key_in_spec in H0 as Hlt.
-    eapply RE.Ext.new_key_add_spec_3 in H0 as H0'.
-    unfold RE.Add in H1.
-    rewrite H1; rewrite H0'. apply RE.valid_update_spec; auto.
-    unfold Cell.valid; simpl. apply well_typed_implies_valid in H2 as [H2 H2']; auto.
-    -- apply instantiation_new in inst as Hnew; now rewrite Hnew in H2.
-    -- apply VContext.valid_empty_spec.
-Qed.
-
 Lemma instantiation_well_typed : forall (Re : ℜ) V (r : resource) (v : 𝑣) (πτ : πΤ),
-  Instᵣₜ(Re,V) -> newᵣᵪ( Re) ⊩ᵣᵪ Re -> Re ⌈ r ⩦ πτ ⌉ᵣᵪ -> V ⌈ r ⩦ v ⌉ᵣᵦ -> 
+  Instᵣₜ(Re,V) -> Re ⌈ r ⩦ πτ ⌉ᵣᵪ -> V ⌈ r ⩦ v ⌉ᵣᵦ -> 
   match (πτ,v) with
     | ((_,τ),⩽ v' … ⩾) => ∅ᵥᵪ ⋅ Re ⊫ v' ∈ τ
     | ((τ,_),⩽ … v' ⩾) => ∅ᵥᵪ ⋅ Re ⊫ v' ∈ τ
   end.
 Proof.
   intros Re V r v πτ inst; revert r v πτ; induction inst;
-  intros r' v' πτ' HvRe HfRe HfV; destruct πτ'.
+  intros r' v' πτ' HfRe HfV; destruct πτ'.
   - apply RC.notEmpty_find_spec in HfRe; auto; contradiction.
-  - rewrite H0 in HfRe; rewrite H1 in HfV.
+  - rewrite H in HfRe; rewrite H0 in HfV.
     apply instantiation_new in inst as Hnew. 
     destruct (Resource.eq_dec (newᵣᵪ(Re)) r'); subst.
-    -- rewrite Hnew in HfV. rewrite RC.add_eq_o in HfRe; auto; 
+    -- rewrite Hnew in HfV. rewrite RC.OP.P.add_eq_o in HfRe; auto; 
         inversion HfRe; clear HfRe; subst.
-        rewrite RE.add_eq_o in HfV; auto; inversion HfV; subst; clear HfV.
-        rewrite <- Hnew. replace 1 with (newᵣᵪ(Re') - newᵣᵪ(Re)).
-        + apply weakening_ℜ_1; auto.
-          ++ apply VContext.valid_empty_spec.
-          ++ apply instantiation_valid in inst as [HvRe' _]; auto.
-          ++ unfold RC.Add in H0. 
-            rewrite H0. apply RC.Submap_add_spec_1.
-            * apply RC.Ext.new_key_notin_spec; lia.
-            * apply RC.Submap_refl.
-        + unfold RC.Add in H0. 
-          rewrite H0; rewrite RC.Ext.new_key_add_new_key_spec; lia.
-    -- rewrite <- Hnew in HfV. rewrite RC.add_neq_o in HfRe; auto.
-        rewrite RE.add_neq_o in HfV; auto.
-        apply instantiation_valid in inst as [HvRe' _].
-        replace r' with ([⧐ᵣ newᵣᵪ(Re) ≤ 1] r') in HfV.
-        + apply RE.shift_find_e_spec in HfV as HfV';
-          destruct HfV' as [v'' Heq]; subst.
-          apply RE.shift_find_spec in HfV.
-          eapply IHinst in HfV; eauto. simpl in HfV.
-          destruct v''; simpl; replace 1 with (newᵣᵪ(Re') - newᵣᵪ(Re));
-          try (apply weakening_ℜ_1); auto; try (apply VContext.valid_empty_spec);
-          unfold RC.Add in H0; rewrite H0; 
-          try ( rewrite RC.Ext.new_key_add_spec_1; auto; try lia ); 
-          try (apply RC.Submap_add_spec_1; try apply RC.Submap_refl);
-          try (apply RC.Ext.new_key_notin_spec; lia). 
-        + rewrite Resource.shift_valid_refl; auto. 
-          eapply RC.valid_find_spec in HfRe; eauto; destruct HfRe; auto.
+        rewrite RE.OP.P.add_eq_o in HfV; auto; inversion HfV; subst; clear HfV.
+        unfold RC.OP.P.Add in H; rewrite H. apply weakening_ℜ with Re; auto.
+        apply RC.Submap_add_spec_1.
+        + apply RC.Ext.new_key_notin_spec; lia.
+        + apply RC.Submap_refl.
+    -- rewrite <- Hnew in HfV. rewrite RC.OP.P.add_neq_o in HfRe; auto.
+        rewrite RE.OP.P.add_neq_o in HfV; auto. eapply IHinst in HfV; eauto.
+        simpl in *; destruct v'.
+        + apply weakening_ℜ with Re; auto; unfold RC.OP.P.Add in H; rewrite H;
+          apply RC.Submap_add_spec_1.
+          ++ apply RC.new_key_notin_spec; lia.
+          ++ apply RC.Submap_refl.
+        + apply weakening_ℜ with Re; auto; unfold RC.OP.P.Add in H; rewrite H;
+          apply RC.Submap_add_spec_1.
+          ++ apply RC.new_key_notin_spec; lia.
+          ++ apply RC.Submap_refl.
   - rewrite H1 in HfV; destruct (Resource.eq_dec r r'); subst.
-    -- rewrite RE.add_eq_o in HfV; auto; inversion HfV; subst; clear HfV.
+    -- rewrite RE.OP.P.add_eq_o in HfV; auto; inversion HfV; subst; clear HfV.
         rewrite H in HfRe; inversion HfRe; subst; auto.
-    -- rewrite RE.add_neq_o in HfV; auto. eapply IHinst in HfV; eauto.
+    -- rewrite RE.OP.P.add_neq_o in HfV; auto. eapply IHinst in HfV; eauto.
         now simpl in HfV.
 Qed.
 
@@ -282,145 +223,24 @@ Lemma instantiation_in : forall (Re : ℜ) V (r : resource),
   Instᵣₜ(Re,V) -> r ∈ᵣᵪ Re <-> r ∈ᵣᵦ V.
 Proof.
   split.
-  - intros; destruct H0; apply RC.find_1 in H0. 
+  - intros; destruct H0; apply RC.OP.P.find_1 in H0. 
     eapply instantiation_domains_match in H0; eauto;
-    destruct H0. exists x0; now apply RE.find_2.
+    destruct H0. exists x0; now apply RE.OP.P.find_2.
   - revert r; induction H.
-    -- intros. unfold RE.Empty in *; exfalso.
+    -- intros. unfold RE.OP.P.Empty in *; exfalso.
        destruct H1. now apply (H0 r x).
-    -- intros. unfold RE.Add in *. rewrite H2 in *.
-       unfold RC.Add in *. rewrite H1.
-       apply RE.add_in_iff in H4; destruct H4; subst.
+    -- intros. unfold RE.OP.P.Add in *. rewrite H1 in *.
+       unfold RC.OP.P.Add in *. rewrite H0.
+       apply RE.OP.P.add_in_iff in H3; destruct H3; subst.
        + apply instantiation_new in H; rewrite H.
-         rewrite RC.add_in_iff; now left.
-       + rewrite RC.add_in_iff; right; apply IHinstantiation_func.
-         rewrite <- RE.valid_in_spec_1; eauto. apply instantiation_valid in H.
-         now destruct H.
-    -- intros. unfold RE.Add in *. rewrite H2 in *. 
-       apply IHinstantiation_func. rewrite RE.add_in_iff in H4.
+         rewrite RC.OP.P.add_in_iff; now left.
+       + rewrite RC.OP.P.add_in_iff; right; now apply IHinstantiation_func.
+    -- intros. unfold RE.OP.P.Add in *. rewrite H2 in *. 
+       apply IHinstantiation_func. rewrite RE.OP.P.add_in_iff in H4.
        destruct H4; subst; auto.
 Qed.
 
 (** ** Preservation *)
-
-Hint Resolve VContext.valid_empty_spec Stock.valid_empty_spec : core.
-
-(** *** Proof of preservation of validity through the functional transition 
-
-  The concept of validity have to be consistent after a functional transition because
-  typing, evaluation transition are based on.
-
-  **** Hypothesis
-
-  If there is a functional transition (1) with the environment (2), the stream term (3) and 
-  the signal function (4) valid according to the new key of the environment;
-
-  **** Result
-
-  All output element of the functional transition (V',st',...) are valid according to the new
-  key of the output environment (5) and the new key of the output environment is greater or equal to the
-  the new key of the input environment (6).
-*)
-Lemma functional_preserves_valid : forall (V V' : 𝓥) (W : 𝐖) (st st' sf sf' : Λ),
-  (* (1) *) ⪡ V ; st ; sf ⪢ ⭆ ⪡ V' ; st' ; sf' ; W ⪢ ->
-  (* (2) *) newᵣᵦ(V) ⊩ᵣᵦ V -> 
-  (* (3) *) newᵣᵦ(V) ⊩ₜₘ st -> 
-  (* (4) *) newᵣᵦ(V) ⊩ₜₘ sf ->
-
-  (* (5) *) newᵣᵦ(V') ⊩ᵣᵦ V' /\ newᵣᵦ(V') ⊩ₜₘ st' /\ newᵣᵦ(V') ⊩ₜₘ sf' /\ newᵣᵦ(V') ⊩ₛₖ W /\ 
-  (* (6) *) newᵣᵦ(V) <= newᵣᵦ(V').
-Proof.
-  intros V V' W st st' sf sf' fT; dependent induction fT; intros HvV Hvst Hvt.
-  (* fT_eT *)
-  - destruct IHfT as [HvV' [Hvst' [Hvt'' [HvW Hlt]]]]; auto.
-    apply evaluate_preserves_valid_term with (t := t); assumption.
-  (* fT_arr *)
-  - split; try assumption; split.
-    -- constructor; inversion Hvt; subst; assumption.
-    -- split; auto; split; try lia. 
-  (* fT_first *)
-  - destruct IHfT as [HvV' [Hvst' [Hvt'' [HvW Hlt]]]]; try assumption.
-    -- apply multi_preserves_valid_term with (t' := <[⟨ v1, v2 ⟩]>) in Hvst as Hvst';
-        try assumption. inversion Hvst'; subst; assumption.
-    -- inversion Hvt; subst; assumption.
-    -- split; try assumption; split.
-        + constructor; try assumption. 
-          apply multi_preserves_valid_term with (t' := <[⟨ v1, v2 ⟩]>) in Hvst as Hvst2;
-          try assumption. inversion Hvst2; subst.
-          apply Term.shift_preserves_valid_1 
-          with (lb := newᵣᵦ(V)) (k' := newᵣᵦ(V') - newᵣᵦ(V)) in H5.
-          replace ((newᵣᵦ(V) + (newᵣᵦ(V') - newᵣᵦ(V)))) with (newᵣᵦ(V')) in H5; auto; lia.
-        + split; constructor; try assumption. inversion Hvt; subst.
-          eapply Typ.valid_weakening; eauto.
-  (* fT_comp *)
-  - inversion Hvt; subst; destruct IHfT1 as [HvV' [Hvst' [Hvt1' [HvW1 Hlt1]]]]; auto.
-    destruct IHfT2 as [HvV'' [Hvst'' [Hvt2' [HvW2 Hlt2]]]]; try assumption.
-    -- apply Term.shift_preserves_valid_1
-        with (lb := newᵣᵦ(V)) (k' := newᵣᵦ(V') - newᵣᵦ(V)) in H4.
-        replace ((newᵣᵦ(V) + (newᵣᵦ(V') - newᵣᵦ(V)))) with (newᵣᵦ(V')) in H4; try assumption; lia.
-    -- split; try assumption; split; auto; split.
-        + constructor; auto; apply Term.shift_preserves_valid_1
-          with (lb := newᵣᵦ(V')) (k' := newᵣᵦ(V'') - newᵣᵦ(V')) in Hvt1'.
-          replace ((newᵣᵦ(V') + (newᵣᵦ(V'') - newᵣᵦ(V')))) with (newᵣᵦ(V'')) in Hvt1';
-          try assumption; lia.
-        + split; try lia. apply Stock.valid_union_spec; split; try assumption.
-          apply Stock.shift_preserves_valid_1 
-          with (lb := newᵣᵦ(V')) (k' := newᵣᵦ(V'') - newᵣᵦ(V')) in HvW1.
-          replace ((newᵣᵦ(V') + (newᵣᵦ(V'') - newᵣᵦ(V')))) with (newᵣᵦ(V'')) in HvW1;
-          try assumption; lia.
-  (* fT_rsf *)
-  - assert (r ∈ᵣᵦ V).
-    { rewrite RE.in_find; rewrite H; intro c; now inversion c. }
-    rewrite RE.Ext.new_key_add_spec_3; try assumption; try lia.
-    split.
-    -- apply RE.valid_update_spec; try assumption.
-    -- split.
-        + apply RE.valid_find_spec with (lb := newᵣᵦ(V)) in H as [_ H]; assumption.
-        + split; auto; split; try lia. 
-  (* fT_wh *)
-  - replace (newᵣᵦ( ⌈ S k ⤆ ⩽ unit … ⩾ ⌉ᵣᵦ (⌈ k ⤆ [⧐ᵣₓ k ≤ 2] ⩽ i … ⩾ ⌉ᵣᵦ ([⧐ᵣᵦ k ≤ 2] V))))
-    with (S (S (newᵣᵦ(V)))) in *.
-    -- inversion Hvt; subst; destruct IHfT as [HvV' [Hvst' [Hvt'' [HvW Hlt]]]]; try assumption. 
-        + apply RE.valid_add_notin_spec.
-          ++ unfold k. apply RE.Ext.new_key_notin_spec.
-            rewrite RE.Ext.new_key_add_spec_1; auto.
-            * apply RE.Ext.new_key_notin_spec; rewrite RE.shift_new_spec; auto.
-            * rewrite RE.shift_new_spec; auto.
-          ++ repeat split.
-            * unfold Resource.valid; lia.
-            * unfold Cell.valid; simpl; constructor.
-            * apply RE.valid_add_notin_spec.
-              ** apply RE.Ext.new_key_notin_spec; 
-                  rewrite RE.shift_new_spec; auto.
-              ** repeat split.
-                  { unfold k,Resource.valid; lia. }
-                  { 
-                  unfold Cell.valid; simpl; replace (S (S (newᵣᵦ(V)))) 
-                  with ((newᵣᵦ(V)) + 2) by lia. now apply Term.shift_preserves_valid_1.  
-                  }
-                  {
-                  unfold Cell.valid; simpl; replace (S (S (newᵣᵦ(V)))) 
-                  with ((newᵣᵦ(V)) + 2) by lia. now apply RE.shift_preserves_valid_1.  
-                  }
-        + replace (S (S (newᵣᵦ(V)))) with ((newᵣᵦ(V)) + 2) by lia.
-          now apply Term.shift_preserves_valid_1.
-        + split; try assumption; split; auto; split; auto; split.
-          ++ apply Stock.valid_add_spec; eauto.
-             * unfold Resource.valid; lia.
-             * inversion Hvt; subst. 
-                  apply Term.shift_preserves_valid_1
-                  with (lb := newᵣᵦ(V)) (k' := newᵣᵦ(V') - newᵣᵦ(V)) in H5.
-                  replace ((newᵣᵦ(V) + (newᵣᵦ(V') - newᵣᵦ(V)))) with (newᵣᵦ(V')) in H5; 
-                  try assumption; lia.
-          ++ lia.
-    -- unfold k; rewrite RE.Ext.new_key_add_spec_1; auto.
-        + apply RE.Ext.new_key_notin_spec; rewrite RE.Ext.new_key_add_spec_1; auto.
-          ++ apply RE.Ext.new_key_notin_spec; rewrite RE.shift_new_spec; lia.
-          ++ rewrite RE.shift_new_spec; lia.
-        + rewrite RE.Ext.new_key_add_spec_1; auto.
-          ++ apply RE.Ext.new_key_notin_spec; rewrite RE.shift_new_spec; lia.
-          ++ rewrite RE.shift_new_spec; lia.
-Qed.
 
 (** *** Proof of preservation of keys in the environment 
 
@@ -428,352 +248,15 @@ Qed.
   needed for the resources environment. Thus, knowing that we cannot loose 
   keys is required.
 *)
-Lemma functional_preserves_keys :  forall (V V' : 𝓥) (W : 𝐖) (sv sv' sf sf' : Λ),
-  ⪡ V ; sv ; sf ⪢ ⭆ ⪡ V' ; sv' ; sf' ; W ⪢ ->
-  newᵣᵦ(V) ⊩ᵣᵦ V -> 
-  newᵣᵦ(V) ⊩ₜₘ sv -> 
-  newᵣᵦ(V) ⊩ₜₘ sf ->
+Lemma functional_preserves_keys (V V' : 𝓥) (tv tv' sf sf' : Λ) :
+  ⪡ V ; tv ; sf ⪢ ⭆ ⪡ V' ; tv' ; sf' ⪢ ->
 
   (forall (r : resource), r ∈ᵣᵦ V -> r ∈ᵣᵦ V').
 Proof.
-  intros V V' W sv sv' sf sf' fT; dependent induction fT; intros HvV Hvsv Hvsf r' HInV; auto.
-  (* fT_eT *)
-  - apply IHfT in HInV; try assumption; eapply evaluate_preserves_valid_term; eauto.
-  (* fT_first *) 
-  - inversion Hvsf; subst; apply IHfT in HInV; auto.
-    eapply multi_preserves_valid_term in H0; try assumption; now inversion H0.
-  (* fT_comp *)
-  - inversion Hvsf; subst. apply IHfT1 in HInV; auto.
-    apply functional_preserves_valid in fT1 as HD; auto; destruct HD as [HvV' [Hvst' [Hvt1' [HvW Hle]]]].
-    apply IHfT2; auto.
-    apply Term.shift_preserves_valid_1 with (lb := newᵣᵦ(V)) (k' := newᵣᵦ(V') - newᵣᵦ(V)) in H4.
-    replace ((newᵣᵦ(V) + (newᵣᵦ(V') - newᵣᵦ(V)))) with (newᵣᵦ(V')) in H4; auto; lia.
+  intros fT; dependent induction fT; intros r' HInV; auto.
   (* fT_rsf *)
-  - destruct (Resource.eq_dec r r'); subst; apply RE.add_in_iff; auto.
-  (* fT_wh *)
-  - replace (newᵣᵦ( ⌈ S k ⤆ ⩽ unit … ⩾ ⌉ᵣᵦ (⌈ k ⤆ [⧐ᵣₓ k ≤ 2] ⩽ i … ⩾ ⌉ᵣᵦ ([⧐ᵣᵦ k ≤ 2] V))))
-    with (S (S (newᵣᵦ(V)))) in *.
-    -- inversion Hvsf; subst; destruct IHfT with (r := r'); auto.
-        + apply RE.valid_add_notin_spec.
-          ++ unfold k. apply RE.Ext.new_key_notin_spec. rewrite RE.Ext.new_key_add_spec_1; auto.
-            * apply RE.Ext.new_key_notin_spec; rewrite RE.shift_new_spec; auto.
-            * rewrite RE.shift_new_spec; auto.
-          ++ repeat split.
-            * unfold Resource.valid; lia.
-            * unfold Cell.valid; simpl; constructor.
-            * apply RE.valid_add_notin_spec.
-              ** apply RE.Ext.new_key_notin_spec; rewrite RE.shift_new_spec; auto.
-              ** repeat split.
-                { unfold k,Resource.valid; lia. }
-                { 
-                  unfold Cell.valid; simpl; replace (S (S (newᵣᵦ(V)))) with ((newᵣᵦ(V)) + 2) by lia.
-                  now apply Term.shift_preserves_valid_1.  
-                }
-                {
-                  unfold Cell.valid; simpl; replace (S (S (newᵣᵦ(V)))) with ((newᵣᵦ(V)) + 2) by lia.
-                  now apply RE.shift_preserves_valid_1.  
-                }
-      + replace (S (S (newᵣᵦ(V)))) with ((newᵣᵦ(V)) + 2) by lia.
-        now apply Term.shift_preserves_valid_1.
-      + destruct (Resource.eq_dec r' (S k)); subst; apply RE.add_in_iff; auto.
-        right; destruct (Resource.eq_dec r' k); subst; apply RE.add_in_iff; auto.
-        right; eapply RE.shift_in_spec in HInV as HInV'.
-        eapply RE.valid_in_spec in HInV; eauto.
-        rewrite Resource.shift_valid_refl in HInV'; eauto.
-      + now exists x.
-    -- unfold k; rewrite RE.Ext.new_key_add_spec_1; auto.
-      + apply RE.Ext.new_key_notin_spec; rewrite RE.Ext.new_key_add_spec_1; auto.
-        ++ apply RE.Ext.new_key_notin_spec; rewrite RE.shift_new_spec; lia.
-        ++ rewrite RE.shift_new_spec; lia.
-      + rewrite RE.Ext.new_key_add_spec_1; auto.
-        ++ apply RE.Ext.new_key_notin_spec; rewrite RE.shift_new_spec; lia.
-        ++ rewrite RE.shift_new_spec; lia.
+  - destruct (Resource.eq_dec r r'); subst; apply RE.OP.P.add_in_iff; auto.
 Qed.
-
-(** *** Proof of consistency between V and W 
-
-  W stocks all virtual resources created during the functional transition. Those virtual
-  resources are also added in the resource environment V' and cannot be found in the environment V.
-*)
-Lemma consistency_V_W : forall (V V' : 𝓥) (W : 𝐖) (sv sv' sf sf' : Λ),
-  ⪡ V ; sv ; sf ⪢ ⭆ ⪡ V' ; sv' ; sf' ; W ⪢ ->
-  newᵣᵦ(V) ⊩ᵣᵦ V -> 
-  newᵣᵦ(V) ⊩ₜₘ sv -> 
-  newᵣᵦ(V) ⊩ₜₘ sf ->
-
-  (forall (r : resource), r ∈ₛₖ W -> r ∉ᵣᵦ V /\ r ∈ᵣᵦ V').
-Proof.
-  intros V V' W sv sv' sf sf' fT; dependent induction fT; intros HvV Hvsv Hvsf; auto.
-  (* fT_eT *)
-  - apply IHfT; try assumption; eapply evaluate_preserves_valid_term; eauto. 
-  (* fT_arr *)
-  - intros. inversion H0; try now inversion H1.
-  (* fT_first *)
-  - intros r HIn; inversion Hvsf; subst; apply IHfT; auto;
-    eapply multi_preserves_valid_term in H0; try assumption; now inversion H0.
-  (* fT_comp *)
-  - inversion Hvsf; subst; intros r HIn.
-    apply functional_preserves_valid in fT1 as HD; auto; destruct HD as [HvV' [Hvst' [Hvt1' [HvW Hle]]]].
-    apply Stock.union_spec in HIn as [HIn | HIn].
-    -- apply Stock.shift_in_e_spec in HIn as Heq'; destruct Heq' as [r' Heq]; subst.
-       apply Stock.shift_in_spec in HIn as HIn'.
-       apply IHfT1 in HIn' as IH; auto.
-       eapply Stock.valid_in_spec in HIn' as Hvr'; eauto.
-       rewrite Resource.shift_valid_refl; auto.
-       destruct IH; split; auto.
-       eapply functional_preserves_keys in H1; eauto.
-        apply Term.shift_preserves_valid_1 with (lb := newᵣᵦ(V)) (k' := newᵣᵦ(V') - newᵣᵦ(V)) in H4;
-        replace ((newᵣᵦ(V) + (newᵣᵦ(V') - newᵣᵦ(V)))) with (newᵣᵦ(V')) in H4; try assumption; lia. 
-    -- apply IHfT2 in HIn; auto.
-       + destruct HIn; split; auto. intro. eapply functional_preserves_keys in H2; eauto.
-       + apply Term.shift_preserves_valid_1 with (lb := newᵣᵦ(V)) (k' := newᵣᵦ(V') - newᵣᵦ(V)) in H4.
-         replace ((newᵣᵦ(V) + (newᵣᵦ(V') - newᵣᵦ(V)))) with (newᵣᵦ(V')) in H4; try assumption; lia.
-  (* fT_rsf *)
-  - intros r' c; exfalso; eapply Stock.empty_in_spec; eauto.
-  (* fT_wh *)
-  - assert (newᵣᵦ( ⌈ S k ⤆ ⩽ unit … ⩾ ⌉ᵣᵦ (⌈ k ⤆ [⧐ᵣₓ k ≤ 2] ⩽ i … ⩾ ⌉ᵣᵦ ([⧐ᵣᵦ k ≤ 2] V)))= (S (S (newᵣᵦ(V))))).
-    {
-      unfold k; rewrite RE.Ext.new_key_add_spec_1; auto.
-        + apply RE.Ext.new_key_notin_spec; rewrite RE.Ext.new_key_add_spec_1; auto.
-          ++ apply RE.Ext.new_key_notin_spec; rewrite RE.shift_new_spec; lia.
-          ++ rewrite RE.shift_new_spec; lia.
-        + rewrite RE.Ext.new_key_add_spec_1; auto.
-          ++ apply RE.Ext.new_key_notin_spec; rewrite RE.shift_new_spec; lia.
-          ++ rewrite RE.shift_new_spec; lia.
-    }
-    inversion Hvsf; subst; intros rf HIn.
-    assert (S (S (newᵣᵦ( V)))
-                      ⊩ᵣᵦ ⌈ S (newᵣᵦ( V)) ⤆ ⩽ unit … ⩾⌉ᵣᵦ (⌈ newᵣᵦ( V) ⤆ [⧐ᵣₓ newᵣᵦ( V) ≤ 2] ⩽ i … ⩾ ⌉ᵣᵦ ([⧐ᵣᵦ newᵣᵦ( V) ≤ 2] V))).
-    {
-      apply RE.valid_add_notin_spec; simpl.
-      + apply RE.Ext.new_key_notin_spec; rewrite RE.Ext.new_key_add_spec_1; auto.
-          * apply RE.Ext.new_key_notin_spec; rewrite RE.shift_new_spec; auto.
-          * rewrite RE.shift_new_spec; auto.
-      + repeat split.
-          * unfold Resource.valid; lia.
-          * unfold Cell.valid; simpl; constructor.
-          * apply RE.valid_add_notin_spec.
-            ** apply RE.Ext.new_key_notin_spec; rewrite RE.shift_new_spec; auto.
-            ** repeat split.
-                { unfold k,Resource.valid; lia. }
-                { 
-                  unfold Cell.valid; simpl; replace (S (S (newᵣᵦ(V)))) with ((newᵣᵦ(V)) + 2) by lia.
-                  now apply Term.shift_preserves_valid_1.
-                }
-                {
-                  unfold Cell.valid; simpl; replace (S (S (newᵣᵦ(V)))) with ((newᵣᵦ(V)) + 2) by lia.
-                  now apply RE.shift_preserves_valid_1.  
-                }
-    }
-    rewrite Stock.add_spec in HIn; destruct HIn as [Heq | [Heq | HIn]]; subst; rewrite H0 in *.
-    -- split.
-       + unfold k. apply RE.Ext.new_key_notin_spec; lia.
-       + simpl; unfold k; eapply functional_preserves_keys; unfold k in *; try rewrite H0; eauto;
-        try ( replace (S (S (newᵣᵦ( V)))) with ((newᵣᵦ( V)) + 2) by lia; now apply Term.shift_preserves_valid_1).
-        rewrite RE.add_in_iff; right; rewrite RE.add_in_iff; now left.
-    -- split.
-       + unfold k. apply RE.Ext.new_key_notin_spec; lia.
-       +  simpl; unfold k; eapply functional_preserves_keys; subst; try rewrite H0; eauto;
-          unfold k in *.
-          ++ replace (S (S (newᵣᵦ( V)))) with ((newᵣᵦ( V)) + 2) by lia; now apply Term.shift_preserves_valid_1.
-          ++ rewrite RE.add_in_iff; now left.
-    -- eapply IHfT in HIn; eauto; unfold k; replace (S (S (newᵣᵦ( V)))) with ((newᵣᵦ( V)) + 2) by lia.
-       + destruct HIn; split; auto. intro c; apply H2. repeat rewrite RE.add_in_iff; repeat right.
-         unfold k. rewrite RE.valid_in_spec_1; auto.
-       + now apply Term.shift_preserves_valid_1.
-Qed.
-
-(** *** Proof of inner constraint of W 
-
-  W stocks reading virtual resource names and writing virtual resource names. It is relevant
-  to state that the intersection of set of reading and writing resource names is empty.
-*)
-Lemma W_well_formed : forall (V V' : 𝓥) (W : 𝐖) (sv sv' sf sf' : Λ),
-  ⪡ V ; sv ; sf ⪢ ⭆ ⪡ V' ; sv' ; sf' ; W ⪢ ->
-  newᵣᵦ(V) ⊩ᵣᵦ V -> 
-  newᵣᵦ(V) ⊩ₜₘ sv -> 
-  newᵣᵦ(V) ⊩ₜₘ sf ->
-
-  (forall r, r ∈ₛₖ W -> (r ∈ᵣₖ (fst W) /\ r ∉ (snd W))%wk \/ (r ∉ᵣₖ (fst W) /\ r ∈ (snd W)))%wk.
-Proof.
-  intros V V' W sv sv' sf sf' fT; dependent induction fT; intros HvV Hvsv Hvsf; auto;
-  try (intros r' c; inversion c; now inversion H0).
-  (* fT_eT *)
-  - intros r HIn. apply IHfT; auto.
-    now apply evaluate_preserves_valid_term with t.
-  (* fT_firts *)
-  - intros; inversion Hvsf; subst; apply IHfT; auto.
-    apply multi_preserves_valid_term in H0; auto; inversion H0; now subst.
-  (* fT_comp *)
-  - intros. rewrite Stock.union_spec in H0; destruct H0.
-    -- inversion Hvsf; subst; eapply functional_preserves_valid in fT1 as Hv; auto.
-       destruct Hv as [HvV' [Hvst' [Hvt1' [HvW Hle]]]].
-       destruct W; unfold Stock.In,Stock.shift in *; simpl in *. inversion HvW.
-       destruct H0. 
-       + left; split; try (rewrite ReadStock.map_union_spec; now left).
-         intro c; rewrite WriteStock.union_spec in *; destruct c.
-         ++ rewrite ReadStock.valid_in_spec_1 in H0; auto.
-            eapply ReadStock.valid_in_spec in H0 as H0'; eauto.
-            replace r with ([⧐ᵣ newᵣᵦ( V') ≤ newᵣᵦ( V'') - newᵣᵦ( V')] r) in H3.
-            * rewrite <- WriteStock.shift_in_spec in H3. 
-              assert (r ∈ᵣₖ t \/ (r ∈ t0)%wk). { now right. }
-              apply IHfT1 in H6; auto; destruct H6; destruct H6; auto.
-            * now apply Resource.shift_valid_refl.
-         ++ rewrite ReadStock.valid_in_spec_1 in H0; auto.
-            assert (r ∈ᵣₖ t \/ (r ∈ t0)%wk). { now left. }
-            eapply consistency_V_W in fT1 as HVW; eauto. destruct HVW as [HnV HV'].
-            destruct W'; simpl in *. 
-            assert (r ∈ᵣₖ t3 \/ (r ∈ t4)%wk). { now right. }
-            eapply consistency_V_W in fT2 as HVW'; eauto.
-            * destruct HVW' as [HnV' HV'']; contradiction.
-            * replace (newᵣᵦ( V')) with (newᵣᵦ( V) + (newᵣᵦ( V') - newᵣᵦ( V))) by lia.
-              apply Term.shift_preserves_valid_3; auto; lia.
-       + simpl in *; right; split; try (rewrite WriteStock.union_spec; now left).
-         rewrite WriteStock.valid_in_spec_1 in H0; auto. intro c.
-         rewrite ReadStock.map_union_spec in *; destruct c.
-         ++ rewrite ReadStock.valid_in_spec_1 in H3; auto.
-            assert (r ∈ᵣₖ t \/ (r ∈ t0)%wk). { now left. }
-            apply IHfT1 in H6; auto; destruct H6; destruct H6; auto.
-         ++ assert (r ∈ᵣₖ t \/ (r ∈ t0)%wk). { now right. }
-            destruct W'; simpl in *. inversion Hvsf; subst.
-            eapply consistency_V_W in fT1 as HVW; eauto; destruct HVW as [HnV HV'].
-            assert (r ∈ᵣₖ t3 \/ (r ∈ t4)%wk). { now left. }
-            eapply consistency_V_W in fT2 as HVW'; eauto.
-            * destruct HVW'; contradiction.
-            * replace (newᵣᵦ( V')) with (newᵣᵦ( V) + (newᵣᵦ( V') - newᵣᵦ( V))) by lia.
-              apply Term.shift_preserves_valid_3; auto; lia.
-    -- inversion Hvsf; subst; eapply functional_preserves_valid in fT1 as Hv; auto.
-       destruct Hv as [HvV' [Hvst' [Hvt1' [HvW Hle]]]].
-       destruct W'; unfold Stock.In in *; simpl in *; destruct H0.
-       + left; split; try (rewrite ReadStock.map_union_spec; now right).
-         intro c. rewrite WriteStock.union_spec in c; destruct c.
-         ++ destruct W; simpl in *; inversion HvW; simpl in *.
-            rewrite WriteStock.valid_in_spec_1 in H1; auto.
-            assert (r ∈ᵣₖ t3 \/ (r ∈ t4)%wk). { now right. }
-            assert (r ∈ᵣₖ t \/ (r ∈ t0)%wk). { now left. }
-            eapply consistency_V_W in fT1; eauto.
-            eapply consistency_V_W in fT2; eauto.
-            * destruct fT1,fT2; contradiction.
-            * replace (newᵣᵦ( V')) with (newᵣᵦ( V) + (newᵣᵦ( V') - newᵣᵦ( V))) by lia.
-              apply Term.shift_preserves_valid_3; auto; lia.
-         ++ assert (r ∈ᵣₖ t \/ (r ∈ t0)%wk). { now right. }
-            apply IHfT2 in H2; auto.
-            * destruct H2; destruct H2; auto.
-            * replace (newᵣᵦ( V')) with (newᵣᵦ( V) + (newᵣᵦ( V') - newᵣᵦ( V))) by lia.
-              apply Term.shift_preserves_valid_3; auto; lia.
-       + right; split; try (rewrite WriteStock.union_spec; now right).
-         intro c. rewrite ReadStock.map_union_spec in c; destruct c.
-         ++ destruct W; simpl in *; inversion HvW; simpl in *.
-            rewrite ReadStock.valid_in_spec_1 in H1; auto.
-            assert (r ∈ᵣₖ t3 \/ (r ∈ t4)%wk). { now left. }
-            assert (r ∈ᵣₖ t \/ (r ∈ t0)%wk). { now right. }
-            eapply consistency_V_W in fT1; eauto.
-            eapply consistency_V_W in fT2; eauto.
-            * destruct fT1,fT2; contradiction.
-            * replace (newᵣᵦ( V')) with (newᵣᵦ( V) + (newᵣᵦ( V') - newᵣᵦ( V))) by lia.
-              apply Term.shift_preserves_valid_3; auto; lia.
-        ++ assert (r ∈ᵣₖ t \/ (r ∈ t0)%wk). { now right. }
-            apply IHfT2 in H2; auto.
-            * destruct H2; destruct H2; auto.
-            * replace (newᵣᵦ( V')) with (newᵣᵦ( V) + (newᵣᵦ( V') - newᵣᵦ( V))) by lia.
-              apply Term.shift_preserves_valid_3; auto; lia.
-  (* fT_wh *)
-  - assert (Heq : RE.Ext.new_key (@RE.Raw.add Cell.t k (Cell.inp (Term.shift k 2 i))
-                            (RE.shift k 2 V)) = S (newᵣᵦ(V))).
-    { 
-      rewrite RE.Ext.new_key_add_spec_1; auto.
-      - apply RE.shift_new_notin_spec; lia.
-      - rewrite RE.shift_new_spec; lia.
-    } 
-    assert (Heq' : RE.Ext.new_key (@RE.Raw.add Cell.raw (S k) (Cell.inp Term.tm_unit)
-                        (@RE.Raw.add Cell.t k (Cell.inp (Term.shift k 2 i))
-                        (RE.shift k 2 V))) = S (S (newᵣᵦ(V)))).
-    { 
-      rewrite RE.Ext.new_key_add_spec_1; auto.
-      - apply RE.Ext.new_key_notin_spec; rewrite Heq; auto.
-      - rewrite RE.Ext.new_key_add_spec_1; auto.
-        -- apply RE.shift_new_notin_spec; lia.
-        -- rewrite RE.shift_new_spec; lia.  
-    }
-    assert (HvshV : S (S (newᵣᵦ(V))) ⊩ᵣᵦ
-                      (@RE.Raw.add Cell.raw (S k) (Cell.inp Term.tm_unit)
-                      (@RE.Raw.add Cell.t k (Cell.inp (Term.shift k 2 i))
-                      (RE.shift k 2 V)))).
-    {
-      apply RE.valid_add_notin_spec.
-      - apply RE.Ext.new_key_notin_spec; rewrite Heq; auto.
-      - repeat split; try constructor. apply RE.valid_add_notin_spec.
-        -- apply RE.shift_new_notin_spec; auto.
-        -- split; try constructor; try lia.
-           + inversion Hvsf; subst. unfold k.
-             replace (S (S (newᵣᵦ( V)))) with ((newᵣᵦ( V)) + 2) by lia.
-             unfold Cell.valid; simpl.
-             now apply Term.shift_preserves_valid_1.
-           + replace (S (S (newᵣᵦ( V)))) with ((newᵣᵦ( V)) + 2) by lia.
-             now apply RE.shift_preserves_valid_1.
-    }
-    intros r HIn. unfold Stock.add, Stock.In in *; destruct W; simpl in *.
-    destruct HIn.
-    -- rewrite ReadStock.add_in_iff in H0; destruct H0; subst.
-       + left; split; try (rewrite ReadStock.add_in_iff; now left).
-         rewrite WriteStock.add_notin_spec; split; try lia.
-         intro c. assert (k ∈ᵣₖ t0 \/ (k ∈ t1)%wk). { now right. }
-         apply IHfT in H0 as H0'.
-         ++ destruct H0'; destruct H1; auto. eapply consistency_V_W in fT; eauto.
-            * apply fT. repeat rewrite RE.add_in_iff; right; now left.
-            * rewrite Heq'; apply HvshV.
-            * rewrite Heq'. replace (S (S (newᵣᵦ( V)))) with ((newᵣᵦ( V)) + 2) by lia.
-              now apply Term.shift_preserves_valid_1.
-            * inversion Hvsf; subst; now rewrite Heq'.
-         ++ rewrite Heq'; apply HvshV.
-         ++ rewrite Heq'. replace (S (S (newᵣᵦ( V)))) with ((newᵣᵦ( V)) + 2) by lia.
-            now apply Term.shift_preserves_valid_1.
-         ++ inversion Hvsf; subst; now rewrite Heq'.
-       + left; split; try (rewrite ReadStock.add_in_iff; now right).
-         rewrite WriteStock.add_notin_spec; split.
-         ++ assert (r ∈ᵣₖ t0 \/ (r ∈ t1)%wk). { now left. }
-            eapply consistency_V_W in fT; eauto.
-            * intro c; subst; apply fT; rewrite RE.add_in_iff; now left.
-            * rewrite Heq'; apply HvshV.
-            * rewrite Heq'. replace (S (S (newᵣᵦ( V)))) with ((newᵣᵦ( V)) + 2) by lia.
-                 now apply Term.shift_preserves_valid_1.
-            * inversion Hvsf; subst; now rewrite Heq'.
-         ++ assert (r ∈ᵣₖ t0 \/ (r ∈ t1)%wk). { now left. } eapply IHfT in H1 as H1'.
-            * destruct H1'; destruct H2; auto.
-            * rewrite Heq'; apply HvshV.
-            * rewrite Heq'. replace (S (S (newᵣᵦ( V)))) with ((newᵣᵦ( V)) + 2) by lia.
-              now apply Term.shift_preserves_valid_1.
-            * inversion Hvsf; subst; now rewrite Heq'.
-    -- rewrite WriteStock.add_spec in H0; destruct H0; subst.
-       + right; split; try (rewrite WriteStock.add_spec; now left).
-         rewrite ReadStock.add_in_iff; intro; destruct H0; try lia.
-         assert ((S k) ∈ᵣₖ t0 \/ ((S k) ∈ t1)%wk). { now left. }
-         eapply consistency_V_W in fT; eauto.
-         ++ apply fT; rewrite RE.add_in_iff; now left.
-         ++ rewrite Heq'; apply HvshV.
-         ++ rewrite Heq'. replace (S (S (newᵣᵦ( V)))) with ((newᵣᵦ( V)) + 2) by lia.
-            now apply Term.shift_preserves_valid_1.
-         ++ inversion Hvsf; subst; now rewrite Heq'.
-       + right; split; try (rewrite WriteStock.add_spec; now right).
-         assert (r ∈ᵣₖ t0 \/ (r ∈ t1)%wk). { now right. }
-         apply IHfT in H1.
-         ++ destruct H1; destruct H1; auto.
-            assert (r ∈ᵣₖ t0 \/ (r ∈ t1)%wk). { now right. }
-            eapply consistency_V_W in fT; eauto.
-            * intro c. apply fT. rewrite RE.add_in_iff;right. 
-              rewrite ReadStock.add_in_iff in c; destruct c; subst;
-              rewrite RE.add_in_iff; auto; contradiction.
-            * rewrite Heq'; apply HvshV.
-            * rewrite Heq'. replace (S (S (newᵣᵦ( V)))) with ((newᵣᵦ( V)) + 2) by lia.
-              now apply Term.shift_preserves_valid_1.
-            * inversion Hvsf; subst; now rewrite Heq'.
-         ++ rewrite Heq'; apply HvshV.
-         ++ rewrite Heq'. replace (S (S (newᵣᵦ( V)))) with ((newᵣᵦ( V)) + 2) by lia.
-            now apply Term.shift_preserves_valid_1.
-         ++ inversion Hvsf; subst; now rewrite Heq'.
-
-Qed.
-
 
 (**
   *** General proof of preservation of typing through functional transition
@@ -790,1148 +273,255 @@ Qed.
   We can state that:
   - each value mapped with a resource name present in R has to be unused (5);
   - each value mapped with a resource name not present in R' but present in V has to be the same in V' (6);
-  - we can found a context and a resource set such as :
-    - the old context is a subset of the new one (7);
-    - the old resources set is a subset of the new one (8);
-    - there is the same property between Re' and V' that between Re and V (9); 
-    - all initial value stocked in W are well typed regards of the new context Re' (10);
-    - all new resources founded in R' are stored in W and is not in R (11); 
-    - Each value mapped with a resource name present in R' has to be used in V' (12);
-    - the output stream term is well typed (13);
-    - the term sf' is well typed (14).
+  - there is the same property between Re and V' that between Re and V (7); 
+  - Each value mapped with a resource name present in R has to be used in V' (8);
+  - the output stream term is well typed (9);
+  - the term sf' is well typed (10).
 
 *)
 Theorem functional_preserves_typing : 
-  forall (Re : ℜ) (V V' : 𝓥) (W : 𝐖) (sv sv' sf sf' : Λ) (τ τ' : Τ) (R : resources),
+  forall (Re : ℜ) (V V' : 𝓥) (tv tv' t t' : Λ) (τ τ' : Τ) (R : resources),
 
-    (* (1) *) ∅ᵥᵪ ⋅ Re ⊫ sf ∈ (τ ⟿ τ' ∣ R) ->
-    (* (2) *) ∅ᵥᵪ ⋅ Re ⊫ sv ∈ τ -> 
-    (* (3) *) ⪡ V ; sv ; sf ⪢ ⭆ ⪡ V' ; sv' ; sf' ; W ⪢ -> 
+    (* (1) *) ∅ᵥᵪ ⋅ Re ⊫ t ∈ (τ ⟿ τ' ∣ R) ->
+    (* (2) *) ∅ᵥᵪ ⋅ Re ⊫ tv ∈ τ -> 
+    (* (3) *) ⪡ V ; tv ; t ⪢ ⭆ ⪡ V' ; tv' ; t' ⪢ -> 
     (* (4) *) Instᵣₜ(Re,V) ->
 
 
     (* (5) *)(forall (r : resource), (r ∈ R)%rs -> RE.unused r V) /\
-    (* (6) *)(forall (r : resource), (r ∉ R)%rs /\ (r ∈ᵣᵦ V) -> 
-                ([⧐ᵣᵦ (newᵣᵦ(V)) ≤ ((newᵣᵦ(V')) - (newᵣᵦ(V)))] V) ⌊r⌋ᵣᵦ = V' ⌊r⌋ᵣᵦ) /\
+    (* (6) *)(forall (r : resource), (r ∉ R)%rs /\ (r ∈ᵣᵦ V) -> V ⌊r⌋ᵣᵦ = V' ⌊r⌋ᵣᵦ) /\
 
-    exists (Re' : ℜ) (R' : resources), 
-      (*  (7) *) Re ⊆ᵣᵪ Re'     /\ 
-      (*  (8) *) (R ⊆ R')%rs    /\
-      (*  (9) *) Instᵣₜ(Re',V') /\
-      (* (10) *) (forall (r : resource) (v : Λ) (τ τ' : Τ), 
-                    W ⌈ r ⩦ v ⌉ₛₖ -> Re' ⌈r ⩦ (τ',τ)⌉ᵣᵪ -> ∅ᵥᵪ ⋅ Re' ⊫ v ∈ τ) /\
-      (* (11) *) (forall (r : resource), (r ∈ (R' \ R))%rs -> (r ∈ (Stock.to_RS W))%rs /\ (r ∉ᵣᵦ V)) /\
-      (* (12) *) (forall (r : resource), (r ∈ R')%rs -> RE.used r V') /\
-      (* (13) *) ∅ᵥᵪ ⋅ Re' ⊫ sv' ∈ τ' /\
-      (* (14) *) ∅ᵥᵪ ⋅ Re' ⊫ sf' ∈ (τ ⟿ τ' ∣ R').
+    (*  (7) *) Instᵣₜ(Re,V') /\
+    (*  (8) *) (forall (r : resource), (r ∈ R)%rs -> RE.used r V') /\
+    (*  (9) *) ∅ᵥᵪ ⋅ Re ⊫ tv' ∈ τ' /\
+    (* (10) *) ∅ᵥᵪ ⋅ Re ⊫ t' ∈ (τ ⟿ τ' ∣ R).
 Proof.
-  intros Re V V' W sv sv' sf sf' τ τ' R Hwsf Hwsv fT; revert Re R τ τ' Hwsf Hwsv;
-  induction fT; intros Re R α β Hwsf Hwsv Hinst;
-
-  apply instantiation_valid in Hinst as HvRe; destruct HvRe as [HvRe HvV];
-  apply instantiation_new in Hinst as Hnew;
-  
-  move HvRe before Hinst; move HvV before HvRe; move Hnew before Hinst.
+  intros Re V V' tv tv' t t' τ τ' R Hwt Hwtv fT. revert Re R τ τ' Hwt Hwtv;
+  induction fT; intros Re R α β Hwt Hwtv Hinst.
   (* fT_eT *)
   - 
     (* clean *)
-    move Re before W; move R before Re; move α before R; move β before α; move fT after IHfT;
+    move R before Re; move α before R; move β before α; move fT after IHfT;
     rename fT into HfT; rename H into HeT; move HeT after HfT.
     (* clean *)
 
-    rewrite <- Hnew in HeT; apply evaluate_preserves_typing with (t' := t') in Hwsf as Hwsf'; 
-    try assumption.
-    
-    (* clean *)
-    clear HeT Hwsf HvRe; move Hwsf' after Hwsv.
-    (* clean *)
-
-    apply IHfT; assumption.
+    apply evaluate_preserves_typing with (t' := t') in Hwt as Hwt'; auto.
   (* fT_arr *)
   - 
     (* clean *)
-    inversion Hwsf; subst; rename H4 into Hwt; clear Hwsf H; move Hwt after Hwsv.
+    inversion Hwt; subst; rename H4 into Hwt'; clear Hwt H; move Hwt' after Hwtv.
     (* clean *)
 
-    repeat split.
+    repeat split; auto.
     -- intros r HIn; inversion HIn.
-    -- intros r [HnIn HIn]; replace (newᵣᵦ(V) - newᵣᵦ(V)) with 0 by lia.
-        now rewrite RE.shift_refl.
-    -- exists Re; exists ∅ᵣₛ; split; try reflexivity.
-        repeat split; auto; try reflexivity; try constructor; auto.
-        + intros; inversion H.
-        + inversion H.
-        + intros r HIn; inversion HIn.
-        + apply wt_app with (τ2 := α); assumption.
+    -- intros r HIn; inversion HIn.
+    -- apply wt_app with (τ2 := α); assumption.
+    -- now constructor.
   (* fT_first *)
   -
     (* clean *)
-    clear H; inversion Hwsf; subst; move Re before W; move R before Re; move τ1 before τ;
-    move τ2 before τ1; clear Hwsf; rename H5 into Hwt; rename H8 into Hvτ;
-    move Hwt after Hwsv; move Hvτ before Hwsv; rename H0 into HmeT; rename fT into HfT;
-    move HfT after IHfT; move HmeT after HfT.
+    clear H; inversion Hwt; subst; move Re before V'; move R before Re; move τ1 before τ;
+    move τ2 before τ1; clear Hwt; rename H3 into Hwt; move Hwt after Hwtv; rename H0 into HmeT; 
+    rename fT into HfT; move HfT after IHfT; move HmeT after HfT.
     (* clean *)
 
-    rewrite <- Hnew in HmeT; apply multi_preserves_typing with (t' := <[⟨v1,v2⟩]>) in Hwsv; 
-    try assumption.
+    apply multi_preserves_typing with (t' := <[⟨v1,v2⟩]>) in Hwtv; auto.
 
     (* clean *)
-    inversion Hwsv; subst; rename H4 into Hwv1; rename H6 into Hwv2; move Hwv1 before Hwt;
-    move Hwv2 before Hwv1; clear Hwsv; move HvRe after Hvτ.
+    inversion Hwtv; subst; rename H4 into Hwv1; rename H6 into Hwv2; move Hwv1 before Hwt;
+    move Hwv2 before Hwv1; clear Hwtv.
     (* clean *)
 
     apply IHfT with (R := R) (τ' := τ2) in Hwv1 as IH; try assumption.
 
-    clear IHfT; destruct IH as [Hunsd [Hlcl [Re' [R' [HSubRe [HSubR [Hinst' [HwtW [HInW [Husd [Hwv1' Hwt']]]]]]]]]]].
+    clear IHfT; destruct IH as [Hunsd [Hlcl [Hinst' [Husd [Hwt1' Hwt']]]]].
 
     (* clean *)
-    move Re' before Re; move R' before R; move Hwv1' before Hwv1; clear Hwv1;
+    move Hwt1' before Hwv1; clear Hwv1; 
     move Hwt' before Hwt; clear Hwt; move Hinst' before Hinst; move Hunsd before Husd.
     (* clean *)
 
-    apply instantiation_new in Hinst' as Hnew'; move Hnew' before Hnew.
-
-    repeat split; auto.
-    exists Re'; exists R'; repeat split; try assumption; try (destruct HSubRe; assumption);
-    try (now apply HInW).
-    -- constructor; try assumption; rewrite <- Hnew; rewrite <- Hnew'; 
-        apply weakening_ℜ_1; auto.
-    -- apply wt_first; try assumption.
-        apply Typ.valid_weakening with (k := newᵣᵪ(Re)); try assumption.
-        apply RC.Ext.new_key_Submap_spec in HSubRe; assumption.
+    repeat split; auto; now constructor.
   (* fT_comp *)
   -
     (* clean *)
-    inversion H; subst; inversion Hwsf; subst; apply Resources.eq_leibniz in H10; subst;
-    clear Hwsf; move Re before W'; move R1 before Re; move R2 before R1; 
+    inversion H; subst; inversion Hwt; subst; apply Resources.eq_leibniz in H10; subst;
+    clear Hwt; move Re before V''; move R1 before Re; move R2 before R1; 
     move α before R2; move β before α; move τ before β; rename fT1 into HfT1;
     move HfT1 after IHfT2; rename fT2 into HfT2; move HfT2 after HfT1.
     rename H9 into Hwt1; rename H11 into Hwt2; rename H12 into HEmp.
-    rename H3 into Hvt2; clear H2; move Hwt1 after Hwsv; move Hwt2 before Hwt1; move Hvt2 after Hwt2.
+    rename H3 into Hvt2; clear H2. move Hwt1 after Hwtv; move Hwt2 before Hwt1; move Hvt2 before Hwtv.
     (* clean *)
 
-    apply IHfT1 with (R := R1) (τ' := τ) in Hwsv as IH1; try assumption;
-    try (intros; apply Hunsd; rewrite Resources.union_spec; now left).
-    clear IHfT1; destruct IH1 as [Hunsd1 [Hlcl1 [Re' [R1' [HSubRe [HSubR1 [Hinst' [HwtW [HInW [Husd1 [Hwsv' Hwt1']]]]]]]]]]].
+    apply IHfT1 with (R := R1) (τ' := τ) in Hwtv as IH1; auto.
+    clear IHfT1; destruct IH1 as [Hunsd1 [Hlcl1 [Hinst' [Husd1 [Hwtv' Hwt1']]]]].
 
     (* clean *)
-    move Re' before Re; move R1' before R1; move Hwsv' before Hwsv;
-    move Hwt1' before Hwt1; move Hunsd1 after HInW; move Hinst' before Hinst.
+    move Hwtv' before Hwtv; move Hwt1' before Hwt1; move Hinst' before Hinst.
     (* clean *)
 
-    apply instantiation_new in Hinst' as Hnew'; move Hnew' before Hnew.
-    apply weakening_ℜ_1 with (Re' := Re') in Hwt2 as Hwt2'; auto; 
-    try now apply VContext.valid_empty_spec.
-    apply IHfT2 with (R := R2) (τ' := β) in Hwsv' as IH2; try assumption;
-    try (rewrite <- Hnew; now rewrite <- Hnew').
-
-    destruct IH2 as [Hunsd2 [Hlcl2 [Re'' [R2' [HSubRe' [HSubR2 [Hinst'' [HwtW' [HInW'  [Husd2 [Hwsv'' Hwt2'']]]]]]]]]]].
+    apply IHfT2 with (R := R2) (τ' := β) in Hwtv' as IH2; auto.
+    clear IHfT2; destruct IH2 as [Hunsd2 [Hlcl2 [Hinst'' [Husd2 [Hwtv'' Hwt2']]]]].
 
     (* clean *)
-    move Re'' before Re'; move R2' before R2; move Hwsv'' before Hwsv';
-    move Hwt2' before Hwt2; move Hwt2'' before Hwt2'; move Hunsd2 before Hunsd1; move Hinst'' before Hinst';
-    clear IHfT2; move HSubRe' before HSubRe; move HSubR2 before HSubR1; move HInW' before HInW;
+    move Hwtv'' before Hwtv'; move Hwt2' before Hwt2; move Hwt2' before Hwt2;
+    move Hunsd2 before Hunsd1; move Hinst'' before Hinst';
     move Husd2 before Husd1; move Hlcl2 before Hlcl1.
     (* clean *)
 
-    assert (HEmp' : (∅ᵣₛ = R1' ∩ R2')%rs).
-    {
-      symmetry; apply Resources.empty_is_empty_1; unfold Resources.Empty.
-      intro r'; intro HIn; rewrite Resources.inter_spec in HIn; 
-      destruct HIn as [HIn1 HIn2].
-      destruct (Resources.In_dec r' R1); destruct (Resources.In_dec r' R2).
-      -- symmetry in HEmp; apply Resources.empty_is_empty_2 in HEmp.
-          unfold Resources.Empty in HEmp; apply (HEmp r').
-          rewrite Resources.inter_spec; split; auto.
-      -- assert (HnInV' : r' ∉ᵣᵦ V'). 
-          { apply HInW'; rewrite Resources.diff_spec; split; assumption. }
-          assert (HInV1 : r' ∈ᵣᵦ V).
-          { 
-          apply Hunsd1 in i; destruct i as [v HfV].  
-          rewrite RE.in_find; intro c; rewrite HfV in *; inversion c.
-          }
+    repeat split; auto.
+    -- intros r HIn; rewrite Resources.union_spec in HIn; destruct HIn; auto.
+       apply Hunsd2 in H0 as Hunsd. destruct Hunsd as [v HfV'].
+       exists v; rewrite Hlcl1; auto; split.
 
-          apply well_typed_implies_valid in Hwt1 as Hv; eauto; 
-          try (apply VContext.valid_empty_spec); destruct Hv as [Hvt1 _].
-          apply well_typed_implies_valid in Hwsv as Hv; eauto; 
-          try (apply VContext.valid_empty_spec); destruct Hv as [Hvsv _].
-          rewrite Hnew in Hvt1,Hvsv.
-          eapply functional_preserves_keys in HInV1; eauto.
-          
-      -- assert (HInV1 : r' ∈ᵣᵦ V).
-          {
-          eapply typing_Re_R in i as HInRe; eauto.
-          eapply instantiation_in in HInRe; eauto. 
-          }
+       + intro; symmetry in HEmp. apply Resources.empty_is_empty_2 in HEmp.
+         apply (HEmp r); rewrite Resources.inter_spec; now split.
+       + eapply typing_Re_R in H0 as HInRe; eauto.
+         eapply instantiation_in in HInRe; eauto. 
 
-          revert HInV1; apply HInW; rewrite Resources.diff_spec; split; assumption.
+    -- intros r [HnIn HIn]; rewrite Resources.union_notin_spec in HnIn; 
+       destruct HnIn as [HnIn1 HnIn2]. rewrite Hlcl1; auto.
+       apply Hlcl2; split; auto. eapply functional_preserves_keys; eauto. 
 
-      -- assert ((r' ∈ Stock.to_RS W)%rs /\ r' ∉ᵣᵦ V).
-          { apply HInW; rewrite Resources.diff_spec; split; assumption. }
-          destruct H0 as [HInW1 HnInV].
-          assert (r' ∉ᵣᵦ V').
-          { apply HInW'; rewrite Resources.diff_spec; split; assumption. }
-          
-          apply well_typed_implies_valid in Hwt1 as Hv; eauto; 
-          try (apply VContext.valid_empty_spec); destruct Hv as [Hvt1 _].
-          apply well_typed_implies_valid in Hwsv as Hv; eauto; 
-          try (apply VContext.valid_empty_spec); destruct Hv as [Hvsv _].
-          rewrite Hnew in Hvt1,Hvsv.
-          
-          apply Stock.to_RS_in_spec in HInW1.
-          eapply consistency_V_W in HfT1; eauto; simpl in *; destruct HfT1; auto.
-      }
+    -- intros r HIn; rewrite Resources.union_spec in HIn; destruct HIn as [HIn | HIn]; auto.
+       assert (HnIn' : (r ∉ R2)%rs). 
+        { 
+          intro. symmetry in HEmp; apply Resources.empty_is_empty_2 in HEmp; 
+          apply (HEmp r); rewrite Resources.inter_spec; split; auto. 
+        }
 
-      move HEmp' before HEmp. repeat split.
-      -- intros r HIn; rewrite Resources.union_spec in HIn; destruct HIn; auto.
-          assert (HInV : r ∈ᵣᵦ V).
-          { eapply typing_Re_R in H0 as HInRe; eauto. eapply instantiation_in in HInRe; eauto. }
+       apply Husd1 in HIn as HuV'; destruct HuV' as [v HfV'].
+       exists v. rewrite <- Hlcl2; auto; split; auto.
+       exists (⩽ … v ⩾); now apply RE.OP.P.find_2.
 
-          assert (HnInR1 : (r ∉ R1)%rs).
-          { 
-            intro; symmetry in HEmp; apply Resources.empty_is_empty_2 in HEmp; 
-            apply (HEmp r); rewrite Resources.inter_spec; now split.
-          }
-
-          destruct HInV as [v HfV]; apply RE.find_1 in HfV; destruct v.
-          + now exists λ.
-          + assert (r ∈ᵣᵦ V). { exists (⩽ … λ ⩾); now apply RE.find_2. }
-          
-            apply RE.shift_find_spec with (lb := newᵣᵦ(V)) (k := newᵣᵦ(V') - newᵣᵦ(V)) in HfV.
-            rewrite Resource.shift_valid_refl in HfV.
-            ++ rewrite Hlcl1 in HfV; try split; auto. apply Hunsd2 in H0; destruct H0; rewrite H0 in *;
-              inversion HfV.
-            ++ eapply RE.valid_in_spec in H1; eauto.
-      -- intros r [HnIn HIn]; rewrite Resources.union_notin_spec in HnIn; destruct HnIn as [HnIn1 HnIn2].
-
-          assert (HIn' : r ∈ᵣᵦ V').
-          { 
-            apply well_typed_implies_valid in Hwt1 as Hv; eauto;
-            try (apply VContext.valid_empty_spec); destruct Hv as [Hvt1 _].
-            apply well_typed_implies_valid in Hwsv as Hv; eauto;
-            try (apply VContext.valid_empty_spec); destruct Hv as [Hvsv _].
-            rewrite Hnew in Hvt1,Hvsv.
-            eapply functional_preserves_keys; eauto. 
-          }
-
-          assert ([⧐ᵣᵦ newᵣᵦ( V) ≤ newᵣᵦ( V'') - newᵣᵦ( V)] V = [⧐ᵣᵦ newᵣᵦ(V') ≤ newᵣᵦ( V'') - newᵣᵦ(V')]([⧐ᵣᵦ newᵣᵦ(V) ≤ newᵣᵦ(V') - newᵣᵦ(V)] V))%re.
-          { 
-            apply RC.Ext.new_key_Submap_spec in HSubRe,HSubRe'.
-            apply instantiation_new in Hinst,Hinst',Hinst''.
-            rewrite Hinst,Hinst' in HSubRe; rewrite Hinst',Hinst'' in HSubRe'.
-            rewrite RE.shift_unfold_1; auto; reflexivity. 
-          }
-
-          rewrite H0; rewrite <- Hlcl2; try (split; auto).
-          destruct HIn as [v HfV]; apply RE.find_1 in HfV.
-          apply RE.shift_find_spec with (lb := newᵣᵦ(V)) (k := newᵣᵦ(V') - newᵣᵦ(V)) in HfV as HfV'.
-
-          apply RE.valid_find_spec with (lb := newᵣᵦ(V)) in HfV as Hv; auto.
-          destruct Hv as [Hvr _]. rewrite Resource.shift_valid_refl in HfV'; auto.
-      
-          apply RE.shift_find_spec with (lb := newᵣᵦ(V')) (k := newᵣᵦ(V'') - newᵣᵦ(V')) in HfV' as HfV''.
-
-          apply instantiation_valid in Hinst' as Hv; destruct Hv as [_ HvV'].
-          apply RE.valid_in_spec with (lb := newᵣᵦ(V')) in HIn' as Hv; auto.
-          rewrite Resource.shift_valid_refl in HfV''; auto. rewrite HfV''. symmetry.
-
-          rewrite <- Resource.shift_valid_refl with (lb := newᵣᵦ(V')) (t := r) (k := newᵣᵦ(V'') - newᵣᵦ(V')); auto.
-          apply RE.shift_find_spec. rewrite <- Hlcl1.
-          + rewrite <- Resource.shift_valid_refl with (lb := newᵣᵦ(V)) (t := r) (k := newᵣᵦ(V') - newᵣᵦ(V)); auto.
-            now apply RE.shift_find_spec.
-          + split; auto. apply RE.in_find; intro c; rewrite HfV in *; inversion c.         
-      -- exists Re''; exists (R1' ∪ R2')%rs; split; try (now transitivity Re'); repeat split; auto.
-          + unfold Resources.Subset; intros r HIn.
-            rewrite Resources.union_spec in *; destruct HIn as [HIn | HIn]; auto.
-          + intros r v τ0 τ' Hfi HfiRe. apply Stock.union_find_spec in Hfi; destruct Hfi.
-            ++ assert (([⧐ₛₖ newᵣᵦ( V') ≤ newᵣᵦ( V'') - newᵣᵦ( V')] W) 
-                            ⌈ ([⧐ᵣ newᵣᵦ( V') ≤ newᵣᵦ( V'') - newᵣᵦ( V')] r) ⩦ v ⌉ₛₖ). 
-               {
-                 assert (r ∈ᵣₖ ([⧐ᵣₖ newᵣᵦ( V') ≤ newᵣᵦ( V'') - newᵣᵦ( V')] (fst W))).
-                 { unfold Stock.find,Stock.shift in *; simpl in *. exists v; now apply ReadStock.find_2. }
-                 apply functional_preserves_valid in HfT1 as H3; auto.
-                 - destruct H3 as [_ [_ [_ [H3 _]]]]. destruct H3.
-                   rewrite ReadStock.valid_in_spec_1 in H1; auto.
-                   eapply ReadStock.valid_in_spec with (lb := newᵣᵦ(V')) in H1; auto.
-                   rewrite Resource.shift_valid_refl; auto.
-                 - apply well_typed_implies_valid in Hwsv; auto.
-                   destruct Hwsv; rewrite <- Hnew; assumption.
-                 - apply well_typed_implies_valid in Hwt1; auto.
-                   destruct Hwt1; rewrite <- Hnew; assumption.
-               }
-               unfold Stock.find,Stock.shift in H1; simpl in *. apply ReadStock.shift_find_e_spec in H1 as H1'.
-               destruct H1'; subst. apply ReadStock.shift_find_spec in H1.
-               eapply HwtW in H1.
-               * rewrite <- Hnew'. 
-                 apply instantiation_new in Hinst''. rewrite <- Hinst''.
-                 apply weakening_ℜ_1; eauto.
-                 apply instantiation_valid in Hinst'. destruct Hinst'; auto.
-               * assert (r ∈ₛₖ W). { unfold Stock.In; left. exists x; now apply ReadStock.find_2. }
-                 eapply consistency_V_W with (r := r) in HfT1 as H3; auto.
-                 ** destruct H3. rewrite <- instantiation_in with (Re := Re') in H4; auto.
-                    destruct H4. apply RC.find_1 in H4. 
-                    apply RC.Submap_find_spec with (m' := Re'') in H4 as H4'; auto.
-                    rewrite HfiRe in H4'; inversion H4'; subst; eauto.
-                 ** apply well_typed_implies_valid in Hwsv; auto.
-                    destruct Hwsv; rewrite <- Hnew; assumption.
-                 ** apply well_typed_implies_valid in Hwt1; auto.
-                    destruct Hwt1; rewrite <- Hnew; assumption. 
-            ++ eapply HwtW'; eauto.
-          + rename H0 into HIn. rewrite Resources.diff_spec in HIn; destruct HIn as [HIn HnIn];
-            rewrite Resources.union_notin_spec in HnIn; destruct HnIn as [HnIn1 HnIn2];
-            rewrite Resources.union_spec in HIn; destruct HIn as [HIn | HIn].
-            ++ assert ((r ∈ Stock.to_RS W)%rs /\ r ∉ᵣᵦ V). { apply HInW; rewrite Resources.diff_spec; now split. }
-              destruct H0.
-               
-              
-              rewrite Stock.to_RS_union_spec; left.
-              apply instantiation_valid in Hinst' as Hv; destruct Hv as [_ HvV'].
-
-              assert (r ∈ᵣᵦ V'). 
-              {
-                apply well_typed_implies_valid in Hwt1 as Hv; eauto; destruct Hv as [Hvt1 _].
-                apply well_typed_implies_valid in Hwsv as Hv; eauto; destruct Hv as [Hvsv _].
-                rewrite Hnew in Hvt1,Hvsv.
-
-                apply Stock.to_RS_in_spec in H0. eapply consistency_V_W in H0; eauto; destruct H0; auto.
-              }
-
-              eapply RE.valid_in_spec in H2; eauto.
-              rewrite <- Resource.shift_valid_refl with (lb := newᵣᵦ(V')) (k := newᵣᵦ(V'') - newᵣᵦ(V')) (t := r); auto.
-              rewrite <- Stock.to_RS_in_spec in *. now apply Stock.shift_in_spec.
-            ++ apply Stock.to_RS_union_spec; right. 
-               apply HInW'; rewrite Resources.diff_spec; split; assumption.
-          + rename H0 into HIn. rewrite Resources.diff_spec in HIn; destruct HIn as [HIn HnIn];
-            rewrite Resources.union_notin_spec in HnIn; destruct HnIn as [HnIn1 HnIn2];
-            rewrite Resources.union_spec in HIn; destruct HIn as [HIn | HIn].
-            ++ apply HInW; rewrite Resources.diff_spec; split; auto. 
-            ++ intro HnInV. assert (HnInV' : r ∉ᵣᵦ V').
-              { apply HInW'; rewrite Resources.diff_spec; split; assumption. }
-              apply HnInV'. 
-              apply well_typed_implies_valid in Hwt1 as Hv; eauto; destruct Hv as [Hvt1 _].
-              apply well_typed_implies_valid in Hwsv as Hv; eauto; destruct Hv as [Hvsv _].
-              rewrite Hnew in Hvt1,Hvsv.
-              eapply functional_preserves_keys; eauto. 
-          + intros r HIn; rewrite Resources.union_spec in HIn; destruct HIn as [HIn | HIn].
-
-            ++ assert (HnIn' : (r ∉ R2')%rs). 
-              { 
-                intro. symmetry in HEmp'; apply Resources.empty_is_empty_2 in HEmp'; 
-                apply (HEmp' r); rewrite Resources.inter_spec; split; auto. 
-              }
-
-              apply Husd1 in HIn as HuV'; destruct HuV' as [v HfV'].
-              apply RE.shift_find_spec with (lb := newᵣᵦ(V')) (k := newᵣᵦ(V'') - newᵣᵦ(V')) in HfV' as HfV''.
-
-              apply instantiation_valid in Hinst' as Hv; destruct Hv as [_ HvV'].
-              rewrite Resource.shift_valid_refl in HfV''; simpl in *.
-          
-              * exists <[[⧐ₜₘ {newᵣᵦ( V')} ≤ {newᵣᵦ( V'') - newᵣᵦ( V')}] v]>. rewrite <- HfV'';
-                symmetry; apply Hlcl2; split; auto; apply RE.in_find;
-                intro c; rewrite HfV' in c; inversion c.
-              * eapply RE.valid_find_spec in HfV'; eauto; now destruct HfV'.
-            ++ apply Husd2 in HIn as HfV'; destruct HfV' as [v HfV']; now exists v.
-          + apply wt_comp with (R1 := R1') (R2 := R2') (τ := τ); try reflexivity; auto.
-            apply instantiation_new in Hinst'' as Hnew''; rewrite <- Hnew'; rewrite <- Hnew''.
-            apply instantiation_valid in Hinst' as HvRe'; destruct HvRe' as [HvRe' _].
-            apply weakening_ℜ_1; auto.
+    -- econstructor; eauto. reflexivity.
   (* fT_rsf *)
   -
     (* clean *)
-    inversion Hwsf; subst. clear Hwsf; move Re before V; rename H into HfV; rename H4 into HfRe;
+    inversion Hwt; subst. clear Hwt; move Re before V; rename H into HfV; rename H4 into HfRe;
     move HfV after HfRe. 
     (* clean *)
 
     repeat split.
     -- intros r' HIn; rewrite Resources.singleton_spec in HIn; subst; now exists v.
     -- intros r' [HnIn HIn]; apply Resources.singleton_notin_spec in HnIn.
-        rewrite RE.add_neq_o; auto. rewrite RE.Ext.new_key_add_spec_3.
-        + replace (newᵣᵦ(V) - newᵣᵦ(V)) with 0 by lia; now rewrite RE.shift_refl.
-        + apply RE.in_find; intro c; rewrite HfV in c; inversion c.
-    -- exists Re; exists \{{r}}; split; try reflexivity. repeat split; try reflexivity.
-        + eapply itfT_update; eauto.
-          ++ apply RE.in_find; intro c; rewrite HfV in c; inversion c.
-          ++ unfold RE.Add; reflexivity.
-        + intros; inversion H.
-        + rename H into HIn; apply Resources.diff_spec in HIn as [HIn HnIn]; contradiction.
-        + rename H into HIn; apply Resources.diff_spec in HIn as [HIn HnIn]; contradiction.
-        + intros r' HIn; apply Resources.singleton_spec in HIn; subst; unfold RE.used.
-          exists st; now apply RE.add_eq_o.
-        + apply instantiation_well_typed with (V := V) (v := ⩽ v … ⩾) in HfRe; try assumption.
-        + apply instantiation_valid in Hinst; destruct Hinst; auto; now constructor.
-  (* fT_wh *)
-  -
-    (* clean *)
-    rename H into Hvwh; inversion Hwsf; subst; move Re before W; move R before Re; move R' before R;
-    move τ before R'; move α before τ; move β before α; unfold k0 in *; 
-    unfold k in *; clear k k0; rename H6 into Hwi; rename H7 into Heq; 
-    rename H8 into Hvα; rename H9 into Hvβ; rename H10 into Hwt;
-    move Hwt after Hwsv; move Hwi after Hwt.
-    (* clean *)
-
-    apply weakening_ℜ_1  with (Re' := ⌈ S (newᵣᵪ( Re)) ⤆ (τ, <[ 𝟙 ]>) ⌉ᵣᵪ 
-                                      (⌈ newᵣᵪ( Re) ⤆ (<[ 𝟙 ]>, τ) ⌉ᵣᵪ Re)) in Hwsv; 
-    auto.
-    -- rewrite RC.new_key_wh_spec in Hwsv.
-        replace (S (S (newᵣᵪ( Re))) - newᵣᵪ( Re)) with 2 in Hwsv by lia. 
-        apply IHfT with (Re :=  ⌈ S (newᵣᵪ( Re)) ⤆ (τ, <[ 𝟙 ]>) ⌉ᵣᵪ 
-                              (⌈ newᵣᵪ( Re) ⤆ (<[ 𝟙 ]>, τ) ⌉ᵣᵪ Re)) (R := R') (τ' := β) in Hwt as IH;
-        auto; try (now rewrite <- Hnew).
-        + clear IHfT; destruct IH as [Hunsd [Hlcl [Re' [R1 [HSubRe [HSubR [Hinst' [HwtW [HInW [Husd [Hwv1' Hwt']]]]]]]]]]].
-
-          repeat split.
-          ++ intros r HIn. assert (HInV : r ∈ᵣᵦ V).
-            { eapply typing_Re_R in Hwsf; eauto. eapply instantiation_in; eauto. }
-
-            rewrite Heq in HIn; rewrite Resources.diff_spec in HIn; destruct HIn.
-            apply Hunsd in H. repeat rewrite Resources.add_notin_spec in H0; destruct H0 as [Hneq [Hneq' _]].
-            destruct H as [v HfV]; rewrite Hnew in Hneq,Hneq'; rewrite RE.add_neq_o in HfV; auto.
-            rewrite RE.add_neq_o in HfV; auto; replace r with ([⧐ᵣ newᵣᵦ(V) ≤ 2] r) in HfV.
-            * apply RE.shift_find_e_spec in HfV as HE. destruct HE as [v' Heq''].
-              destruct v'; simpl in Heq''; inversion Heq''; subst; exists λ.
-              eapply RE.shift_find_spec; eauto.
-            * apply Resource.shift_valid_refl. eapply RE.valid_in_spec; eauto. 
-          ++ intros r [HnIn HIn]; rewrite Heq in HnIn. rewrite Resources.diff_notin_spec in HnIn;
-            destruct HnIn as [HnIn | HIn'].
-            * simpl in Hlcl; symmetry. rewrite <- Hlcl.
-              ** transitivity (([⧐ᵣᵦ (newᵣᵦ(V) + 2) ≤ newᵣᵦ( V') - (newᵣᵦ(V) + 2)] 
-                            ⌈ S (newᵣᵦ( V)) ⤆ ⩽ unit … ⩾⌉ᵣᵦ (⌈ newᵣᵦ( V) ⤆ ⩽ [⧐ₜₘ{newᵣᵦ( V)} ≤ 2] i … ⩾ ⌉ᵣᵦ ([⧐ᵣᵦ newᵣᵦ( V) ≤ 2] V))) ⌊ r ⌋ᵣᵦ).
-                  {
-                  assert (newᵣᵦ( ⌈ S (newᵣᵦ(V)) ⤆ ⩽ unit … ⩾ ⌉ᵣᵦ 
-                          (⌈ newᵣᵦ(V) ⤆ ⩽ [⧐ₜₘ {newᵣᵦ(V)} ≤ 2] i … ⩾ ⌉ᵣᵦ ([⧐ᵣᵦ newᵣᵦ(V) ≤ 2] V))) =  newᵣᵦ(V) + 2).
-                  { 
-                    rewrite RE.Ext.new_key_add_spec_1; try lia.
-                    + apply RE.Ext.new_key_notin_spec; rewrite RE.Ext.new_key_add_spec_1; try lia.
-                      ++ apply RE.shift_new_notin_spec; eauto.
-                      ++ rewrite RE.shift_new_spec; lia.
-                    + rewrite RE.Ext.new_key_add_spec_1; try lia.
-                      ++ apply RE.shift_new_notin_spec; lia.
-                      ++ rewrite RE.shift_new_spec; lia.
-                  } 
-                  f_equal; f_equal; f_equal; assumption.
-                  }
-                  {
-                  rewrite RE.shift_add_notin_spec.
-                  - rewrite RE.add_neq_o.
-                    -- rewrite RE.shift_add_notin_spec.
-                        + rewrite RE.add_neq_o.
-                          ++ rewrite <- RE.shift_unfold. f_equal; f_equal.
-                            apply RC.Ext.new_key_Submap_spec in HSubRe. rewrite RC.new_key_wh_spec in HSubRe.
-                              rewrite Hnew in HSubRe. apply instantiation_new in Hinst'; rewrite Hinst' in HSubRe; lia.
-                          ++ intro; subst. rewrite Resource.shift_valid_refl in HIn by (unfold Resource.valid; lia).
-                            revert HIn; apply RE.Ext.new_key_notin_spec; lia.
-                        + apply RE.shift_new_notin_spec; lia.
-                    -- intro; subst. rewrite Resource.shift_valid_refl in HIn by (unfold Resource.valid; lia).
-                        revert HIn; apply RE.Ext.new_key_notin_spec; lia.
-                  - apply RE.Ext.new_key_notin_spec; rewrite RE.Ext.new_key_add_spec_1; auto.
-                    -- apply RE.shift_new_notin_spec; lia.
-                    -- rewrite RE.shift_new_spec; auto.
-                  }
-              ** split; auto. repeat rewrite RE.add_in_iff; repeat right.
-                  eapply RE.shift_in_spec in HIn as HIn'; rewrite Resource.shift_valid_refl in HIn';
-                  eauto; eapply RE.valid_in_spec in HIn; eauto. 
-            * repeat rewrite Resources.add_spec in HIn'; destruct HIn' as [Heq' | [Heq' | HIn']];
-              try (now inversion HIn); subst; rewrite Hnew in HIn; clear Hnew; exfalso;
-              revert HIn; apply RE.Ext.new_key_notin_spec; lia.
-          ++ exists Re'; exists R1.
-            split.
-            { 
-              apply RC.Submap_Add_spec with (m := (⌈ newᵣᵪ( Re) ⤆ (<[ 𝟙 ]>, τ) ⌉ᵣᵪ Re))
-                                              (x := S (newᵣᵪ( Re))) (v := (τ, <[ 𝟙 ]>)) in HSubRe; eauto.
-              - apply RC.Submap_Add_spec with
-                  (m := Re) (x := newᵣᵪ( Re)) (v := (<[ 𝟙 ]>, τ)) in HSubRe; eauto.
-                -- apply RC.Ext.new_key_notin_spec; auto.
-                -- unfold RC.Add;  reflexivity.
-              - intro c. rewrite RC.add_in_iff in c; destruct c; try lia.
-                revert H; apply RC.Ext.new_key_notin_spec; lia.
-              - unfold RC.Add; reflexivity.
-            }
-            repeat split; auto.
-            * unfold Resources.Subset; intros r' HIn. rewrite Heq in HIn. 
-              rewrite Resources.diff_spec in HIn; destruct HIn. now apply HSubR.
-            * intros r v τ0 τ' Hfi Hfi'. unfold Stock.find,Stock.add in Hfi; simpl in *.
-              destruct (Resource.eq_dec r (newᵣᵦ(V))); subst.
-              ** rewrite ReadStock.add_eq_o in Hfi; auto; inversion Hfi.
-                 apply instantiation_new in Hinst'; rewrite <- Hinst'. rewrite <- Hnew.
-                 apply weakening_ℜ_1; eauto.
-                 { 
-                  eapply RC.Submap_Add_spec with (x := (newᵣᵪ(Re))) 
-                                                       (v := (<[ 𝟙 ]>, τ))
-                                                       (m':= (⌈ newᵣᵪ( Re) ⤆ (<[ 𝟙 ]>, τ) ⌉ᵣᵪ Re)); eauto.
-                  - eapply RC.Submap_Add_spec with (x := S (newᵣᵪ(Re))); eauto.
-                    -- apply RC.Ext.new_key_notin_spec. rewrite RC.Ext.new_key_add_spec_1; eauto.
-                       apply RC.Ext.new_key_notin_spec; lia.
-                    -- unfold RC.Add; reflexivity.
-                  - apply RC.Ext.new_key_notin_spec; lia.
-                  - unfold RC.Add; reflexivity.
-                 }
-                 { 
-                  eapply RC.Submap_find_spec with (x := (newᵣᵪ(Re))) (v := (<[ 𝟙 ]>, τ)) in HSubRe. 
-                  - rewrite  <- Hnew in Hfi'. rewrite HSubRe in Hfi'; inversion Hfi'; now subst.
-                  - rewrite RC.add_neq_o; try lia; rewrite RC.add_eq_o; auto.   
-                 }
-              ** rewrite ReadStock.add_neq_o in Hfi; auto. eapply HwtW; eauto.
-            * rename H into HIn. rewrite Resources.diff_spec in HIn.
-              destruct HIn as [HIn HnIn]. rewrite Heq in HnIn; rewrite Resources.diff_notin_spec in HnIn.
-              destruct HnIn as [HnIn | HIn'].
-              ** assert (r ∈ R1 \ R')%rs. { rewrite Resources.diff_spec; split; assumption. }
-                  apply HInW in H as [HInW1 HnInV]. rewrite <- Stock.to_RS_in_spec in *.
-                  rewrite Stock.add_spec; simpl; auto.
-              ** apply Stock.to_RS_in_spec. apply Stock.add_spec; auto; repeat rewrite Resources.add_spec in HIn'; 
-                  destruct HIn' as [Heq' | [Heq' | HIn']]; try (now inversion HIn'); subst; 
-                  apply instantiation_new in Hinst; rewrite <- Hinst; simpl; auto.
-            * rename H into HIn. rewrite Resources.diff_spec in HIn.
-              destruct HIn as [HIn HnIn]. rewrite Heq in HnIn; rewrite Resources.diff_notin_spec in HnIn.
-              destruct HnIn as [HnIn | HIn'].
-              ** assert (r ∈ R1 \ R')%rs. { rewrite Resources.diff_spec; split; assumption. }
-                  apply HInW in H as [HInW1 HnInV]; intro c; apply HnInV. 
-                  repeat rewrite RE.add_in_iff; repeat right.
-                  eapply RE.shift_in_spec in c as c'; rewrite Resource.shift_valid_refl in c'; eauto.
-                  eapply RE.valid_in_spec in c; eauto.
-              ** rewrite Hnew in HIn'. repeat rewrite Resources.add_spec in HIn'; 
-                  destruct HIn' as [Heq' | [Heq' | HIn']]; try (inversion HIn'); subst; 
-                  apply RE.Ext.new_key_notin_spec; lia.
-        + replace 2 with (1 + 1) by lia. rewrite Cell.shift_unfold.
-          replace ((newᵣᵦ(V)) + 1) with (S (newᵣᵦ(V))) by lia. 
-
-          assert (RE.eq ([⧐ᵣᵦ (newᵣᵦ(V)) ≤ 1 + 1] V) ([⧐ᵣᵦ S (newᵣᵦ(V)) ≤ 1] [⧐ᵣᵦ (newᵣᵦ(V)) ≤ 1] V)).
-          { rewrite RE.shift_unfold; replace ((newᵣᵦ(V)) + 1) with (S (newᵣᵦ(V))) by lia; reflexivity. }
-          rewrite H.
-      
-          assert (RE.eq (⌈ (newᵣᵦ(V)) ⤆ [⧐ᵣₓ S (newᵣᵦ(V)) ≤ 1] [⧐ᵣₓ (newᵣᵦ(V)) ≤ 1] ⩽ i … ⩾ ⌉ᵣᵦ ([⧐ᵣᵦ S (newᵣᵦ(V)) ≤ 1] [⧐ᵣᵦ (newᵣᵦ(V)) ≤ 1] V))
-                              ([⧐ᵣᵦ S (newᵣᵦ(V)) ≤ 1] (⌈ (newᵣᵦ(V)) ⤆ [⧐ᵣₓ (newᵣᵦ(V)) ≤ 1] ⩽ i … ⩾ ⌉ᵣᵦ ([⧐ᵣᵦ (newᵣᵦ(V)) ≤ 1] V)))).
-          { 
-            rewrite RE.shift_add_notin_spec.
-            - replace ([⧐ᵣ S (newᵣᵦ(V)) ≤ 1] (newᵣᵦ(V))) with (newᵣᵦ(V)); try reflexivity.
-              rewrite Resource.shift_valid_refl; auto; unfold Resource.valid; lia.
-            - apply RE.shift_new_notin_spec; lia.
-          }
-          rewrite H0. clear H H0.
-          eapply (itfT_init 
-                    (⌈ newᵣᵪ( Re) ⤆ (<[ 𝟙 ]>, τ) ⌉ᵣᵪ Re)
-                    (⌈ S (newᵣᵪ( Re)) ⤆ (τ, <[ 𝟙 ]>) ⌉ᵣᵪ (⌈ newᵣᵪ( Re) ⤆ (<[ 𝟙 ]>, τ) ⌉ᵣᵪ Re))
-                    (⌈ newᵣᵦ( V) ⤆ [⧐ᵣₓ newᵣᵦ( V) ≤ 1] ⩽ i … ⩾ ⌉ᵣᵦ ([⧐ᵣᵦ newᵣᵦ( V) ≤ 1] V))
-                    (⌈ S (newᵣᵦ( V)) ⤆ ⩽ unit … ⩾ ⌉ᵣᵦ ([⧐ᵣᵦ S (newᵣᵦ( V)) ≤ 1] ⌈ newᵣᵦ( V) ⤆ [⧐ᵣₓ newᵣᵦ( V) ≤ 1] ⩽ i … ⩾ ⌉ᵣᵦ ([⧐ᵣᵦ newᵣᵦ( V) ≤ 1] V)))
-                    τ <[𝟙]> <[unit]>); eauto; try now constructor.
-          ++ eapply (itfT_init Re (⌈ newᵣᵪ( Re) ⤆ (<[ 𝟙 ]>, τ) ⌉ᵣᵪ Re)
-                                  V (⌈ newᵣᵦ( V) ⤆ [⧐ᵣₓ newᵣᵦ( V) ≤ 1] ⩽ i … ⩾ ⌉ᵣᵦ ([⧐ᵣᵦ newᵣᵦ( V) ≤ 1] V))
-                                  <[𝟙]> τ); eauto; try constructor.
-          ++ rewrite RC.Ext.new_key_add_spec_1; auto.
-              * apply well_typed_implies_valid in Hwi; auto.
-                destruct Hwi; apply Typ.valid_weakening with (k := newᵣᵪ( Re)); auto.
-              * apply RC.Ext.new_key_notin_spec; auto.
-          ++ unfold RC.Add;
-            rewrite RC.Ext.new_key_add_spec_1; auto; try reflexivity.
-            apply RC.Ext.new_key_notin_spec; auto.
-          ++ unfold RE.Add;
-            rewrite RE.Ext.new_key_add_spec_1; auto; try reflexivity.
-            * apply RE.shift_new_notin_spec; lia.
-            * rewrite RE.shift_new_spec; auto.
-    -- apply RC.Submap_add_spec_1.
-        + apply RC.Ext.new_key_notin_spec; rewrite RC.Ext.new_key_add_spec_1;
-          auto. apply RC.Ext.new_key_notin_spec; lia.
-        + apply RC.Submap_add_spec_1.
-          ++ apply RC.Ext.new_key_notin_spec; lia.
-          ++ apply RC.Submap_refl.
+       rewrite RE.OP.P.add_neq_o; auto.
+    -- eapply itfT_update; eauto.
+       + apply RE.OP.P.in_find; intro c; rewrite HfV in c; inversion c.
+       + unfold RE.OP.P.Add; reflexivity.
+    -- intros r' HIn; apply Resources.singleton_spec in HIn; subst; unfold RE.used.
+       exists st; now apply RE.OP.P.add_eq_o.
+    -- apply instantiation_well_typed with (V := V) (v := ⩽ v … ⩾) in HfRe; try assumption.
+    -- now constructor.
 Qed.
 
 
-(**
-  *** General proof of preservation of typing value through functional transition
+(** ** Progress *)
 
-  This proof is almost the same as above with the difference that the signal function expression
-  is a value. Knowing that we can state that if all expression on the environment and the stream 
-  expression can be normalised then the output expressions in V' and the output stream expression
-  can also be normalised.
-  
-  _This proof stands only if we can find a property that state that all arrow functions foundable in the signal function expression have all possible applications normalisable_. 
 
-*)
-Theorem functional_preserves_typing_value : 
-  forall (Re : ℜ) (V V' : 𝓥) (W : 𝐖) (sv sv' sf sf' : Λ) (τ τ' : Τ) (R : resources),
-
-    ∅ᵥᵪ ⋅ Re ⊫ sf ∈ (τ ⟿ τ' ∣ R) ->
-    value(sf) ->
-    ∅ᵥᵪ ⋅ Re ⊫ sv ∈ τ -> 
-    ⪡ V ; sv ; sf ⪢ ⭆ ⪡ V' ; sv' ; sf' ; W ⪢ -> 
+Theorem progress_of_functional_value (Re : ℜ) (V : 𝓥) (tv t : Λ) (τ τ' : Τ) (R : resources) :
+    halts tv ->
+    RE.halts V ->
+    all_arrow_halting ->
+    value(t) -> 
+    
+    ∅ᵥᵪ ⋅ Re ⊫ t ∈ (τ ⟿ τ' ∣ R) -> 
+    ∅ᵥᵪ ⋅ Re ⊫ tv ∈ τ ->
     Instᵣₜ(Re,V) ->
-    RE.halts (newᵣᵦ(V)) V ->
-    halts (newᵣᵪ(Re)) sv ->
 
-
-    (forall (r : resource), (r ∈ R)%rs -> RE.unused r V) /\
-    (forall (r : resource), (r ∉ R)%rs /\ (r ∈ᵣᵦ V) -> 
-                ([⧐ᵣᵦ (newᵣᵦ(V)) ≤ ((newᵣᵦ(V')) - (newᵣᵦ(V)))] V) ⌊r⌋ᵣᵦ = V' ⌊r⌋ᵣᵦ) /\
-
-    exists (Re' : ℜ) (R' : resources), 
-      Re ⊆ᵣᵪ Re'     /\ 
-      (R ⊆ R')%rs    /\
-      Instᵣₜ(Re',V') /\
-
-      RE.halts (newᵣᵦ(V')) V' /\
-      halts (newᵣᵪ(Re')) sv' /\
-
-      (forall (r : resource) (v : Λ) (τ τ' : Τ), 
-                    W ⌈ r ⩦ v ⌉ₛₖ -> Re' ⌈r ⩦ (τ',τ)⌉ᵣᵪ -> ∅ᵥᵪ ⋅ Re' ⊫ v ∈ τ) /\
-      (forall (r : resource), (r ∈ (R' \ R))%rs -> (r ∈ (Stock.to_RS W))%rs /\ (r ∉ᵣᵦ V)) /\
-      (forall (r : resource), (r ∈ R')%rs -> RE.used r V') /\
-      ∅ᵥᵪ ⋅ Re' ⊫ sv' ∈ τ' /\
-      ∅ᵥᵪ ⋅ Re' ⊫ sf' ∈ (τ ⟿ τ' ∣ R').
+    (exists (V' : 𝓥) (tv' : Λ), 
+      ⪡ V ; tv ; t ⪢ ⭆ ⪡ V' ; tv' ; t ⪢ /\
+      halts tv' /\
+      RE.halts V').
 Proof.
-  intros Re V V' W sv sv' sf sf' τ τ' R Hwsf Hvsf Hwsv fT; revert Re R τ τ' Hwsf Hvsf Hwsv;
-  induction fT; intros Re R α β Hwsf Hvsf Hwsv Hinst HltV Hltst;
-
-  apply instantiation_valid in Hinst as HvRe; destruct HvRe as [HvRe HvV];
-  apply instantiation_new in Hinst as Hnew;
-
-  move HvRe before Hinst; move HvV before HvRe; move Hnew before Hinst.
-  (* fT_eT *)
-  - apply evaluate_not_value in H; contradiction. 
-  (* fT_arr *)
-  - 
-    (* clean *)
-    inversion Hwsf; subst; rename H4 into Hwt; clear Hwsf H; move Hwt after Hwsv.
-    (* clean *)
-
-    repeat split.
-    -- intros r HIn; inversion HIn.
-    -- intros r [HnIn HIn]; replace (newᵣᵦ(V) - newᵣᵦ(V)) with 0 by lia.
-        now rewrite RE.shift_refl.
-    -- exists Re; exists ∅ᵣₛ; split; try reflexivity.
-        repeat split; auto; try reflexivity; try constructor; auto.
-        + admit. 
-          (* 
-            Add a new property that state that every arrow block has a function
-            that finished for all normalisable well-typed expression 
-          *)
-        + intros; inversion H.
-        + inversion H.
-        + intros r HIn; inversion HIn.
-        + apply wt_app with (τ2 := α); assumption.
-  (* fT_first *)
+  intros Hltv HltV HlAll Hvt wt; revert V tv Hltv HltV HlAll Hvt.
+  dependent induction wt; intros V tv Hltv HltV HlAll Hvt Hwtv Hinst; inversion Hvt; subst.
+  (* wt-arr *)
   -
     (* clean *)
-    clear H; inversion Hwsf; subst; move Re before W; move R before Re; move τ1 before τ;
-    move τ2 before τ1; clear Hwsf; rename H5 into Hwt; rename H8 into Hvτ;
-    move Hwt after Hwsv; move Hvτ before Hwsv; rename H0 into HmeT; rename fT into HfT;
-    move HfT after IHfT; move HmeT after HfT.
+    clear Hvt; rename H0 into Hvt; move V before Re; move tv before t; clear IHwt.
     (* clean *)
 
-    rewrite <- Hnew in HmeT; apply multi_preserves_typing with (t' := <[⟨v1,v2⟩]>) in Hwsv; 
-    try assumption.
-
-    (* clean *)
-    inversion Hwsv; subst; rename H4 into Hwv1; rename H6 into Hwv2; move Hwv1 before Hwt;
-    move Hwv2 before Hwv1; clear Hwsv; move HvRe after Hvτ; inversion Hvsf; subst;
-    clear Hvsf; rename H0 into Hvsf.
-    (* clean *)
-
-    rewrite multi_preserves_halting in Hltst; eauto. rewrite halts_pair in Hltst.
-    destruct Hltst as [Hltv1 Hltv2].
-    apply IHfT with (R := R) (τ' := τ2) in Hwv1 as IH; try assumption.
-
-    clear IHfT; 
-    destruct IH as [Hunsd [Hlcl [Re' [R' [HSubRe [HSubR [Hinst' [HltV' [Hltv1' 
-                            [HwtW [HInW [Husd [Hwv1' Hwt']]]]]]]]]]]]].
-
-    (* clean *)
-    move Re' before Re; move R' before R; move Hwv1' before Hwv1; clear Hwv1;
-    move Hwt' before Hwt; clear Hwt; move Hinst' before Hinst; move Hunsd before Husd.
-    (* clean *)
-
-    apply instantiation_new in Hinst' as Hnew'; move Hnew' before Hnew.
-
-    repeat split; auto.
-    exists Re'; exists R'; repeat split; try assumption; try (destruct HSubRe; assumption);
-    try (now apply HInW).
-    -- rewrite halts_pair; split; auto. rewrite <- Hnew; rewrite <- Hnew'.
-       apply halts_weakening; auto. now apply RC.Ext.new_key_Submap_spec.
-    -- constructor; try assumption; rewrite <- Hnew; rewrite <- Hnew'; 
-        apply weakening_ℜ_1; auto.
-    -- apply wt_first; try assumption.
-        apply Typ.valid_weakening with (k := newᵣᵪ(Re)); try assumption.
-        apply RC.Ext.new_key_Submap_spec in HSubRe; assumption.
-  (* fT_comp *)
+    exists V; exists <[t tv]>; repeat split; auto.
+    -- now repeat constructor.
+    -- unfold all_arrow_halting in HlAll; apply (HlAll Re _ τ τ'); auto. 
+       now constructor.
+  (* wt-first *)
   -
     (* clean *)
-    inversion H; subst; inversion Hwsf; subst; apply Resources.eq_leibniz in H10; subst;
-    clear Hwsf; move Re before W'; move R1 before Re; move R2 before R1; 
-    move α before R2; move β before α; move τ before β; rename fT1 into HfT1;
-    move HfT1 after IHfT2; rename fT2 into HfT2; move HfT2 after HfT1.
-    rename H9 into Hwt1; rename H11 into Hwt2; rename H12 into HEmp.
-    rename H3 into Hvt2; clear H2; move Hwt1 after Hwsv; move Hwt2 before Hwt1; move Hvt2 after Hwt2.
-    inversion Hvsf; subst; clear Hvsf; rename H2 into Hvlt1; rename H3 into Hvlt2.
+    clear Hvt; rename H0 into Hvt; move V before Re; move tv before t.
     (* clean *)
 
-    apply IHfT1 with (R := R1) (τ' := τ) in Hwsv as IH1; try assumption;
-    try (intros; apply Hunsd; rewrite Resources.union_spec; now left).
-    clear IHfT1; destruct IH1 as [Hunsd1 [Hlcl1 [Re' [R1' [HSubRe [HSubR1 
-                                    [Hinst' [HltV' [Hltst' [HwtW [HInW [Husd1 [Hwsv' Hwt1']]]]]]]]]]]]].
+    destruct Hltv as [tv' [HmeT Hvtv']].
+    apply multi_preserves_typing with (t' := tv') in Hwtv as Hwtv'; auto.
+    destruct tv'; subst; inversion Hwtv'; subst; inversion Hvtv'; subst.
 
     (* clean *)
-    move Re' before Re; move R1' before R1; move Hwsv' before Hwsv;
-    move Hwt1' before Hwt1; move Hunsd1 after HInW; move Hinst' before Hinst.
+    clear Hwtv Hwtv' Hvtv'; rename H4 into Hwtv'1; rename H6 into Hwtv'2.
+    rename H1 into Hvtv'1; rename H2 into Hvtv'2. move wt before Hwtv'1. move Hvt before Hvtv'1.
+    move tv'1 before tv; move tv'2 before tv'1.
     (* clean *)
 
-    apply instantiation_new in Hinst' as Hnew'; move Hnew' before Hnew.
-    apply weakening_ℜ_1 with (Re' := Re') in Hwt2 as Hwt2'; auto.
-    apply IHfT2 with (R := R2) (τ' := β) in Hwsv' as IH2; try assumption;
-    try (rewrite <- Hnew; now rewrite <- Hnew');
-    try (now apply Term.shift_value_iff).
+    eapply IHwt in Hwtv'1 as IH; eauto; clear IHwt.
+    -- destruct IH as [V' [tv''1 [HfT [Hltv''1 HltV']]]].
+       exists V'; exists <[⟨tv''1,tv'2⟩]>; repeat split; auto.
+       + eapply fT_first; eauto.
+       + apply halts_pair; split; auto. exists tv'2; auto.
+    -- exists tv'1; split; auto.
+  (* wt-comp *)
+  - admit.
+  (* wt-rsf *)
+  - (* Il faut des garanti sur l'état des valeurs associé à tout r dans R dans V. *)
+ Admitted.
 
-    destruct IH2 as [Hunsd2 [Hlcl2 [Re'' [R2' [HSubRe' [HSubR2 [Hinst'' 
-                                              [HltV'' [Hltst'' [HwtW' [HInW'  [Husd2 [Hwsv'' Hwt2'']]]]]]]]]]]]].
+Theorem progress_of_functional(Re : ℜ) (V : 𝓥) (tv t : Λ) (τ τ' : Τ) (R : resources) : 
+  halts t -> halts tv -> RE.halts V ->
+  all_arrow_halting ->
+
+  ∅ᵥᵪ ⋅ Re ⊫ t ∈ (τ ⟿ τ' ∣ R) -> 
+  ∅ᵥᵪ ⋅ Re ⊫ tv ∈ τ ->
+  Instᵣₜ(Re,V) ->
+
+  (exists (V' : 𝓥) (tv' t' : Λ), 
+    ⪡ V ; tv ; t ⪢ ⭆ ⪡ V' ; tv' ; t' ⪢ /\
+    halts t' /\ halts tv'/\ RE.halts V'
+  ).
+Proof. 
+  intros Hlt; destruct Hlt as [t' [HmeT Hvt']]. apply multi_indexed in HmeT as [k HieT].
+  revert Re V tv t τ τ' R t' HieT Hvt'. induction k; 
+  intros Re V tv t τ τ' R t' HieT Hvt' Hltv HltV HltAll Hwt Hwtv Hinst.
+  (* sf is a value *)
+  - inversion HieT; subst. 
+    apply (progress_of_functional_value _ _ tv t' τ τ' R) in Hinst; try assumption.
+    destruct Hinst as [V' [tv' [HfT [Hltv' HltV']]]].
+    exists V'; exists tv'; exists t'; repeat split; auto.
+    exists t'; split; auto.
+  (* sf can be reduced at least one time *)
+  - inversion HieT; subst.
 
     (* clean *)
-    move Re'' before Re'; move R2' before R2; move Hwsv'' before Hwsv';
-    move Hwt2' before Hwt2; move Hwt2'' before Hwt2'; move Hunsd2 before Hunsd1; move Hinst'' before Hinst';
-    clear IHfT2; move HSubRe' before HSubRe; move HSubR2 before HSubR1; move HInW' before HInW;
-    move Husd2 before Husd1; move Hlcl2 before Hlcl1.
+    clear HieT; rename y into t1; rename H0 into HeT; rename H1 into HieT.
+    move t1 before t; move t' before t.
     (* clean *)
 
-    assert (HEmp' : (∅ᵣₛ = R1' ∩ R2')%rs).
-    {
-      symmetry; apply Resources.empty_is_empty_1; unfold Resources.Empty.
-      intro r'; intro HIn; rewrite Resources.inter_spec in HIn; 
-      destruct HIn as [HIn1 HIn2].
-      destruct (Resources.In_dec r' R1); destruct (Resources.In_dec r' R2).
-      -- symmetry in HEmp; apply Resources.empty_is_empty_2 in HEmp.
-          unfold Resources.Empty in HEmp; apply (HEmp r').
-          rewrite Resources.inter_spec; split; auto.
-      -- assert (HnInV' : r' ∉ᵣᵦ V'). 
-          { apply HInW'; rewrite Resources.diff_spec; split; assumption. }
-          assert (HInV1 : r' ∈ᵣᵦ V).
-          { 
-          apply Hunsd1 in i; destruct i as [v HfV].  
-          rewrite RE.in_find; intro c; rewrite HfV in *; inversion c.
-          }
-
-          apply well_typed_implies_valid in Hwt1 as Hv; eauto; destruct Hv as [Hvt1 _].
-          apply well_typed_implies_valid in Hwsv as Hv; eauto; destruct Hv as [Hvsv _].
-          rewrite Hnew in Hvt1,Hvsv.
-          eapply functional_preserves_keys in HInV1; eauto.
-          
-      -- assert (HInV1 : r' ∈ᵣᵦ V).
-          {
-          eapply typing_Re_R in i as HInRe; eauto.
-          eapply instantiation_in in HInRe; eauto. 
-          }
-
-          revert HInV1; apply HInW; rewrite Resources.diff_spec; split; assumption.
-
-      -- assert ((r' ∈ Stock.to_RS W)%rs /\ r' ∉ᵣᵦ V).
-          { apply HInW; rewrite Resources.diff_spec; split; assumption. }
-          destruct H0 as [HInW1 HnInV].
-          assert (r' ∉ᵣᵦ V').
-          { apply HInW'; rewrite Resources.diff_spec; split; assumption. }
-          
-          apply well_typed_implies_valid in Hwt1 as Hv; eauto; destruct Hv as [Hvt1 _].
-          apply well_typed_implies_valid in Hwsv as Hv; eauto; destruct Hv as [Hvsv _].
-          rewrite Hnew in Hvt1,Hvsv.
-          
-          apply Stock.to_RS_in_spec in HInW1.
-          eapply consistency_V_W in HfT1; eauto; simpl in *; destruct HfT1; auto.
-      }
-
-      move HEmp' before HEmp. repeat split.
-      -- intros r HIn; rewrite Resources.union_spec in HIn; destruct HIn; auto.
-          assert (HInV : r ∈ᵣᵦ V).
-          { eapply typing_Re_R in H0 as HInRe; eauto. eapply instantiation_in in HInRe; eauto. }
-
-          assert (HnInR1 : (r ∉ R1)%rs).
-          { 
-            intro; symmetry in HEmp; apply Resources.empty_is_empty_2 in HEmp; 
-            apply (HEmp r); rewrite Resources.inter_spec; now split.
-          }
-
-          destruct HInV as [v HfV]; apply RE.find_1 in HfV; destruct v.
-          + now exists λ.
-          + assert (r ∈ᵣᵦ V). { exists (⩽ … λ ⩾); now apply RE.find_2. }
-          
-            apply RE.shift_find_spec with (lb := newᵣᵦ(V)) (k := newᵣᵦ(V') - newᵣᵦ(V)) in HfV.
-            rewrite Resource.shift_valid_refl in HfV.
-            ++ rewrite Hlcl1 in HfV; try split; auto. apply Hunsd2 in H0; destruct H0; rewrite H0 in *;
-              inversion HfV.
-            ++ eapply RE.valid_in_spec in H1; eauto.
-      -- intros r [HnIn HIn]; rewrite Resources.union_notin_spec in HnIn; destruct HnIn as [HnIn1 HnIn2].
-
-          assert (HIn' : r ∈ᵣᵦ V').
-          { 
-            apply well_typed_implies_valid in Hwt1 as Hv; eauto; destruct Hv as [Hvt1 _].
-            apply well_typed_implies_valid in Hwsv as Hv; eauto; destruct Hv as [Hvsv _].
-            rewrite Hnew in Hvt1,Hvsv.
-            eapply functional_preserves_keys; eauto. 
-          }
-
-          assert ([⧐ᵣᵦ newᵣᵦ( V) ≤ newᵣᵦ( V'') - newᵣᵦ( V)] V = [⧐ᵣᵦ newᵣᵦ(V') ≤ newᵣᵦ( V'') - newᵣᵦ(V')]([⧐ᵣᵦ newᵣᵦ(V) ≤ newᵣᵦ(V') - newᵣᵦ(V)] V))%re.
-          { 
-            apply RC.Ext.new_key_Submap_spec in HSubRe,HSubRe'.
-            apply instantiation_new in Hinst,Hinst',Hinst''.
-            rewrite Hinst,Hinst' in HSubRe; rewrite Hinst',Hinst'' in HSubRe'.
-            rewrite RE.shift_unfold_1; auto; reflexivity. 
-          }
-
-          rewrite H0; rewrite <- Hlcl2; try (split; auto).
-          destruct HIn as [v HfV]; apply RE.find_1 in HfV.
-          apply RE.shift_find_spec with (lb := newᵣᵦ(V)) (k := newᵣᵦ(V') - newᵣᵦ(V)) in HfV as HfV'.
-
-          apply RE.valid_find_spec with (lb := newᵣᵦ(V)) in HfV as Hv; auto.
-          destruct Hv as [Hvr _]. rewrite Resource.shift_valid_refl in HfV'; auto.
-      
-          apply RE.shift_find_spec with (lb := newᵣᵦ(V')) (k := newᵣᵦ(V'') - newᵣᵦ(V')) in HfV' as HfV''.
-
-          apply instantiation_valid in Hinst' as Hv; destruct Hv as [_ HvV'].
-          apply RE.valid_in_spec with (lb := newᵣᵦ(V')) in HIn' as Hv; auto.
-          rewrite Resource.shift_valid_refl in HfV''; auto. rewrite HfV''. symmetry.
-
-          rewrite <- Resource.shift_valid_refl with (lb := newᵣᵦ(V')) (t := r) (k := newᵣᵦ(V'') - newᵣᵦ(V')); auto.
-          apply RE.shift_find_spec. rewrite <- Hlcl1.
-          + rewrite <- Resource.shift_valid_refl with (lb := newᵣᵦ(V)) (t := r) (k := newᵣᵦ(V') - newᵣᵦ(V)); auto.
-            now apply RE.shift_find_spec.
-          + split; auto. apply RE.in_find; intro c; rewrite HfV in *; inversion c.         
-      -- exists Re''; exists (R1' ∪ R2')%rs; split; try (now transitivity Re'); repeat split; auto.
-          + unfold Resources.Subset; intros r HIn.
-            rewrite Resources.union_spec in *; destruct HIn as [HIn | HIn]; auto.
-          + intros r v τ0 τ' Hfi HfiRe. apply Stock.union_find_spec in Hfi; destruct Hfi.
-            ++ assert (([⧐ₛₖ newᵣᵦ( V') ≤ newᵣᵦ( V'') - newᵣᵦ( V')] W) 
-                            ⌈ ([⧐ᵣ newᵣᵦ( V') ≤ newᵣᵦ( V'') - newᵣᵦ( V')] r) ⩦ v ⌉ₛₖ). 
-              {
-                assert (r ∈ᵣₖ ([⧐ᵣₖ newᵣᵦ( V') ≤ newᵣᵦ( V'') - newᵣᵦ( V')] (fst W))).
-                { unfold Stock.find,Stock.shift in *; simpl in *. exists v; now apply ReadStock.find_2. }
-                apply functional_preserves_valid in HfT1 as H3; auto.
-                - destruct H3 as [_ [_ [_ [H3 _]]]]. destruct H3.
-                  rewrite ReadStock.valid_in_spec_1 in H1; auto.
-                  eapply ReadStock.valid_in_spec with (lb := newᵣᵦ(V')) in H1; auto.
-                  rewrite Resource.shift_valid_refl; auto.
-                - apply well_typed_implies_valid in Hwsv; auto.
-                  destruct Hwsv; rewrite <- Hnew; assumption.
-                - apply well_typed_implies_valid in Hwt1; auto.
-                  destruct Hwt1; rewrite <- Hnew; assumption.
-              }
-              unfold Stock.find,Stock.shift in H1; simpl in *. apply ReadStock.shift_find_e_spec in H1 as H1'.
-              destruct H1'; subst. apply ReadStock.shift_find_spec in H1.
-              eapply HwtW in H1.
-              * rewrite <- Hnew'. 
-                apply instantiation_new in Hinst''. rewrite <- Hinst''.
-                apply weakening_ℜ_1; eauto.
-                apply instantiation_valid in Hinst'. destruct Hinst'; auto.
-              * assert (r ∈ₛₖ W). { unfold Stock.In; left. exists x; now apply ReadStock.find_2. }
-                eapply consistency_V_W with (r := r) in HfT1 as H3; auto.
-                ** destruct H3. rewrite <- instantiation_in with (Re := Re') in H4; auto.
-                    destruct H4. apply RC.find_1 in H4. 
-                    apply RC.Submap_find_spec with (m' := Re'') in H4 as H4'; auto.
-                    rewrite HfiRe in H4'; inversion H4'; subst; eauto.
-                ** apply well_typed_implies_valid in Hwsv; auto.
-                    destruct Hwsv; rewrite <- Hnew; assumption.
-                ** apply well_typed_implies_valid in Hwt1; auto.
-                    destruct Hwt1; rewrite <- Hnew; assumption. 
-            ++ eapply HwtW'; eauto.
-          + rename H0 into HIn. rewrite Resources.diff_spec in HIn; destruct HIn as [HIn HnIn];
-            rewrite Resources.union_notin_spec in HnIn; destruct HnIn as [HnIn1 HnIn2];
-            rewrite Resources.union_spec in HIn; destruct HIn as [HIn | HIn].
-            ++ assert ((r ∈ Stock.to_RS W)%rs /\ r ∉ᵣᵦ V). { apply HInW; rewrite Resources.diff_spec; now split. }
-              destruct H0.
-              
-              
-              rewrite Stock.to_RS_union_spec; left.
-              apply instantiation_valid in Hinst' as Hv; destruct Hv as [_ HvV'].
-
-              assert (r ∈ᵣᵦ V'). 
-              {
-                apply well_typed_implies_valid in Hwt1 as Hv; eauto; destruct Hv as [Hvt1 _].
-                apply well_typed_implies_valid in Hwsv as Hv; eauto; destruct Hv as [Hvsv _].
-                rewrite Hnew in Hvt1,Hvsv.
-
-                apply Stock.to_RS_in_spec in H0. eapply consistency_V_W in H0; eauto; destruct H0; auto.
-              }
-
-              eapply RE.valid_in_spec in H2; eauto.
-              rewrite <- Resource.shift_valid_refl with (lb := newᵣᵦ(V')) (k := newᵣᵦ(V'') - newᵣᵦ(V')) (t := r); auto.
-              rewrite <- Stock.to_RS_in_spec in *. now apply Stock.shift_in_spec.
-            ++ apply Stock.to_RS_union_spec; right. 
-              apply HInW'; rewrite Resources.diff_spec; split; assumption.
-          + rename H0 into HIn. rewrite Resources.diff_spec in HIn; destruct HIn as [HIn HnIn];
-            rewrite Resources.union_notin_spec in HnIn; destruct HnIn as [HnIn1 HnIn2];
-            rewrite Resources.union_spec in HIn; destruct HIn as [HIn | HIn].
-            ++ apply HInW; rewrite Resources.diff_spec; split; auto. 
-            ++ intro HnInV. assert (HnInV' : r ∉ᵣᵦ V').
-              { apply HInW'; rewrite Resources.diff_spec; split; assumption. }
-              apply HnInV'. 
-              apply well_typed_implies_valid in Hwt1 as Hv; eauto; destruct Hv as [Hvt1 _].
-              apply well_typed_implies_valid in Hwsv as Hv; eauto; destruct Hv as [Hvsv _].
-              rewrite Hnew in Hvt1,Hvsv.
-              eapply functional_preserves_keys; eauto. 
-          + intros r HIn; rewrite Resources.union_spec in HIn; destruct HIn as [HIn | HIn].
-
-            ++ assert (HnIn' : (r ∉ R2')%rs). 
-              { 
-                intro. symmetry in HEmp'; apply Resources.empty_is_empty_2 in HEmp'; 
-                apply (HEmp' r); rewrite Resources.inter_spec; split; auto. 
-              }
-
-              apply Husd1 in HIn as HuV'; destruct HuV' as [v HfV'].
-              apply RE.shift_find_spec with (lb := newᵣᵦ(V')) (k := newᵣᵦ(V'') - newᵣᵦ(V')) in HfV' as HfV''.
-
-              apply instantiation_valid in Hinst' as Hv; destruct Hv as [_ HvV'].
-              rewrite Resource.shift_valid_refl in HfV''; simpl in *.
-          
-              * exists <[[⧐ₜₘ {newᵣᵦ( V')} ≤ {newᵣᵦ( V'') - newᵣᵦ( V')}] v]>. rewrite <- HfV'';
-                symmetry; apply Hlcl2; split; auto; apply RE.in_find;
-                intro c; rewrite HfV' in c; inversion c.
-              * eapply RE.valid_find_spec in HfV'; eauto; now destruct HfV'.
-            ++ apply Husd2 in HIn as HfV'; destruct HfV' as [v HfV']; now exists v.
-          + apply wt_comp with (R1 := R1') (R2 := R2') (τ := τ); try reflexivity; auto.
-            apply instantiation_new in Hinst'' as Hnew''; rewrite <- Hnew'; rewrite <- Hnew''.
-            apply instantiation_valid in Hinst' as HvRe'; destruct HvRe' as [HvRe' _].
-            apply weakening_ℜ_1; auto.
-  (* fT_rsf *)
-  -
-    (* clean *)
-    inversion Hwsf; subst. clear Hwsf; move Re before V; rename H into HfV; rename H4 into HfRe;
-    move HfV after HfRe. 
-    (* clean *)
-
-    repeat split.
-    -- intros r' HIn; rewrite Resources.singleton_spec in HIn; subst; now exists v.
-    -- intros r' [HnIn HIn]; apply Resources.singleton_notin_spec in HnIn.
-        rewrite RE.add_neq_o; auto. rewrite RE.Ext.new_key_add_spec_3.
-        + replace (newᵣᵦ(V) - newᵣᵦ(V)) with 0 by lia; now rewrite RE.shift_refl.
-        + apply RE.in_find; intro c; rewrite HfV in c; inversion c.
-    -- exists Re; exists \{{r}}; split; try reflexivity. repeat split; try reflexivity.
-        + eapply itfT_update; eauto.
-          ++ apply RE.in_find; intro c; rewrite HfV in c; inversion c.
-          ++ unfold RE.Add; reflexivity.
-        + apply RE.halts_add_spec; split.
-          ++ rewrite RE.Ext.new_key_add_spec_3; simpl.
-             * now rewrite <- Hnew.
-             * exists (⩽ v … ⩾); now apply RE.find_2.
-          ++ rewrite RE.Ext.new_key_add_spec_3; auto. exists (⩽ v … ⩾); now apply RE.find_2.
-        + rewrite Hnew; destruct (HltV r (⩽ v … ⩾)); auto.
-          now exists x. 
-        + intros; inversion H.
-        + rename H into HIn; apply Resources.diff_spec in HIn as [HIn HnIn]; contradiction.
-        + rename H into HIn; apply Resources.diff_spec in HIn as [HIn HnIn]; contradiction.
-        + intros r' HIn; apply Resources.singleton_spec in HIn; subst; unfold RE.used.
-          exists st; now apply RE.add_eq_o.
-        + apply instantiation_well_typed with (V := V) (v := ⩽ v … ⩾) in HfRe; try assumption.
-        + apply instantiation_valid in Hinst; destruct Hinst; auto; now constructor.
-  (* fT_wh *)
-  -
-    (* clean *)
-    rename H into Hvwh; inversion Hwsf; subst; move Re before W; move R before Re; move R' before R;
-    move τ before R'; move α before τ; move β before α; unfold k0 in *; 
-    unfold k in *; clear k k0; rename H6 into Hwi; rename H7 into Heq; 
-    rename H8 into Hvα; rename H9 into Hvβ; rename H10 into Hwt;
-    move Hwt after Hwsv; move Hwi after Hwt.
-    inversion Hvsf; subst; clear Hvsf; rename H1 into Hvli; rename H2 into Hvl2.
-    (* clean *)
-
-    assert (Heqnk : (RE.Ext.new_key
-      (@RE.Raw.add Cell.t (RE.Ext.new_key V) (Cell.shift (RE.Ext.new_key V) 2 (Cell.inp i))
-      (RE.shift (RE.Ext.new_key V) 2 V))) = S (RE.Ext.new_key V)).
-    { 
-      rewrite RE.Ext.new_key_add_spec_1; auto.
-      - apply RE.shift_new_notin_spec; auto.
-      - rewrite RE.shift_new_spec; lia. 
-    }
-
-    assert (Heqnk' : (RE.Ext.new_key
-    (@RE.Raw.add Cell.raw (S (RE.Ext.new_key V)) (Cell.inp Term.tm_unit)
-       (@RE.Raw.add Cell.t (RE.Ext.new_key V) (Cell.shift (RE.Ext.new_key V) 2 (Cell.inp i))
-          (RE.shift (RE.Ext.new_key V) 2 V)))) = S (S (RE.Ext.new_key V))).
-    {
-      rewrite RE.Ext.new_key_add_spec_1; auto.
-      - apply RE.Ext.new_key_notin_spec; rewrite Heqnk; auto.
-      - rewrite Heqnk; lia.
-    }
-
-    apply weakening_ℜ_1  with (Re' := ⌈ S (newᵣᵪ( Re)) ⤆ (τ, <[ 𝟙 ]>) ⌉ᵣᵪ 
-                                      (⌈ newᵣᵪ( Re) ⤆ (<[ 𝟙 ]>, τ) ⌉ᵣᵪ Re)) in Hwsv; 
-    auto.
-    -- rewrite RC.new_key_wh_spec in Hwsv.
-        replace (S (S (newᵣᵪ( Re))) - newᵣᵪ( Re)) with 2 in Hwsv by lia. 
-        apply IHfT with (Re :=  ⌈ S (newᵣᵪ( Re)) ⤆ (τ, <[ 𝟙 ]>) ⌉ᵣᵪ 
-                              (⌈ newᵣᵪ( Re) ⤆ (<[ 𝟙 ]>, τ) ⌉ᵣᵪ Re)) (R := R') (τ' := β) in Hwt as IH;
-        auto; try (now rewrite <- Hnew).
-        + clear IHfT; 
-          destruct IH as [Hunsd [Hlcl [Re' [R1 [HSubRe [HSubR [Hinst' 
-                                    [HltV' [Hltv1' [HwtW [HInW [Husd [Hwv1' Hwt']]]]]]]]]]]]].
-
-          rewrite Heqnk' in *; repeat split.
-          ++ intros r HIn. assert (HInV : r ∈ᵣᵦ V).
-            { eapply typing_Re_R in Hwsf; eauto. eapply instantiation_in; eauto. }
-
-            rewrite Heq in HIn; rewrite Resources.diff_spec in HIn; destruct HIn.
-            apply Hunsd in H. repeat rewrite Resources.add_notin_spec in H0; destruct H0 as [Hneq [Hneq' _]].
-            destruct H as [v HfV]; rewrite Hnew in Hneq,Hneq'; rewrite RE.add_neq_o in HfV; auto.
-            rewrite RE.add_neq_o in HfV; auto; replace r with ([⧐ᵣ newᵣᵦ(V) ≤ 2] r) in HfV.
-            * apply RE.shift_find_e_spec in HfV as HE. destruct HE as [v' Heq''].
-              destruct v'; simpl in Heq''; inversion Heq''; subst; exists λ.
-              eapply RE.shift_find_spec; eauto.
-            * apply Resource.shift_valid_refl. eapply RE.valid_in_spec; eauto. 
-          ++ intros r [HnIn HIn]; rewrite Heq in HnIn. rewrite Resources.diff_notin_spec in HnIn;
-            destruct HnIn as [HnIn | HIn'].
-            * symmetry. rewrite <- Hlcl.
-              ** transitivity (([⧐ᵣᵦ (newᵣᵦ(V) + 2) ≤ newᵣᵦ( V') - (newᵣᵦ(V) + 2)] 
-                            ⌈ S (newᵣᵦ( V)) ⤆ ⩽ unit … ⩾⌉ᵣᵦ (⌈ newᵣᵦ( V) ⤆ [⧐ᵣₓ (newᵣᵦ(V)) ≤ 2] ⩽ i … ⩾ ⌉ᵣᵦ ([⧐ᵣᵦ newᵣᵦ(V) ≤ 2] V))) ⌊ r ⌋ᵣᵦ).
-                  { f_equal; f_equal; try lia. }
-                  {
-                  rewrite RE.shift_add_notin_spec.
-                  - rewrite RE.add_neq_o.
-                    -- rewrite RE.shift_add_notin_spec.
-                        + rewrite RE.add_neq_o.
-                          ++ rewrite <- RE.shift_unfold. f_equal; f_equal.
-                            apply RC.Ext.new_key_Submap_spec in HSubRe. rewrite RC.new_key_wh_spec in HSubRe.
-                              rewrite Hnew in HSubRe. apply instantiation_new in Hinst'; rewrite Hinst' in HSubRe; lia.
-                          ++ intro; subst. rewrite Resource.shift_valid_refl in HIn by (unfold Resource.valid; lia).
-                            revert HIn; apply RE.Ext.new_key_notin_spec; lia.
-                        + apply RE.shift_new_notin_spec; lia.
-                    -- intro; subst. rewrite Resource.shift_valid_refl in HIn by (unfold Resource.valid; lia).
-                        revert HIn; apply RE.Ext.new_key_notin_spec; lia.
-                  - apply RE.Ext.new_key_notin_spec. rewrite Heqnk; auto.
-                  }
-              ** split; auto. repeat rewrite RE.add_in_iff; repeat right.
-                  eapply RE.shift_in_spec in HIn as HIn'; rewrite Resource.shift_valid_refl in HIn';
-                  eauto; eapply RE.valid_in_spec in HIn; eauto. 
-            * repeat rewrite Resources.add_spec in HIn'; destruct HIn' as [Heq' | [Heq' | HIn']];
-              try (now inversion HIn); subst; rewrite Hnew in HIn; clear Hnew; exfalso;
-              revert HIn; apply RE.Ext.new_key_notin_spec; lia.
-          ++ exists Re'; exists R1.
-            split.
-            { 
-              apply RC.Submap_Add_spec with (m := (⌈ newᵣᵪ( Re) ⤆ (<[ 𝟙 ]>, τ) ⌉ᵣᵪ Re))
-                                              (x := S (newᵣᵪ( Re))) (v := (τ, <[ 𝟙 ]>)) in HSubRe; eauto.
-              - apply RC.Submap_Add_spec with
-                  (m := Re) (x := newᵣᵪ( Re)) (v := (<[ 𝟙 ]>, τ)) in HSubRe; eauto.
-                -- apply RC.Ext.new_key_notin_spec; auto.
-                -- unfold RC.Add; reflexivity.
-              - intro c. rewrite RC.add_in_iff in c; destruct c; try lia.
-                revert H; apply RC.Ext.new_key_notin_spec; lia.
-              - unfold RC.Add; reflexivity.
-            }
-            repeat split; auto.
-            * unfold Resources.Subset; intros r' HIn. rewrite Heq in HIn. 
-              rewrite Resources.diff_spec in HIn; destruct HIn. now apply HSubR.
-            * intros r v τ0 τ' Hfi Hfi'. unfold Stock.find,Stock.add in Hfi; simpl in *.
-              destruct (Resource.eq_dec r (newᵣᵦ(V))); subst.
-              ** rewrite ReadStock.add_eq_o in Hfi; auto; inversion Hfi.
-                apply instantiation_new in Hinst'; rewrite <- Hinst'. rewrite <- Hnew.
-                apply weakening_ℜ_1; eauto.
-                { 
-                  eapply RC.Submap_Add_spec with (x := (newᵣᵪ(Re))) 
-                                                      (v := (<[ 𝟙 ]>, τ))
-                                                      (m':= (⌈ newᵣᵪ( Re) ⤆ (<[ 𝟙 ]>, τ) ⌉ᵣᵪ Re)); eauto.
-                  - eapply RC.Submap_Add_spec with (x := S (newᵣᵪ(Re))); eauto.
-                    -- apply RC.Ext.new_key_notin_spec. rewrite RC.Ext.new_key_add_spec_1; eauto.
-                      apply RC.Ext.new_key_notin_spec; lia.
-                    -- unfold RC.Add; reflexivity.
-                  - apply RC.Ext.new_key_notin_spec; lia.
-                  - unfold RC.Add. reflexivity.
-                }
-                { 
-                  eapply RC.Submap_find_spec with (x := (newᵣᵪ(Re))) (v := (<[ 𝟙 ]>, τ)) in HSubRe. 
-                  - rewrite  <- Hnew in Hfi'. rewrite HSubRe in Hfi'; inversion Hfi'; now subst.
-                  - rewrite RC.add_neq_o; try lia; rewrite RC.add_eq_o; auto.   
-                }
-              ** rewrite ReadStock.add_neq_o in Hfi; auto. eapply HwtW; eauto.
-            * rename H into HIn. rewrite Resources.diff_spec in HIn.
-              destruct HIn as [HIn HnIn]. rewrite Heq in HnIn; rewrite Resources.diff_notin_spec in HnIn.
-              destruct HnIn as [HnIn | HIn'].
-              ** assert (r ∈ R1 \ R')%rs. { rewrite Resources.diff_spec; split; assumption. }
-                  apply HInW in H as [HInW1 HnInV]. rewrite <- Stock.to_RS_in_spec in *.
-                  rewrite Stock.add_spec; simpl; auto.
-              ** apply Stock.to_RS_in_spec. apply Stock.add_spec; auto; repeat rewrite Resources.add_spec in HIn'; 
-                  destruct HIn' as [Heq' | [Heq' | HIn']]; try (now inversion HIn'); subst; 
-                  apply instantiation_new in Hinst; rewrite <- Hinst; simpl; auto.
-            * rename H into HIn. rewrite Resources.diff_spec in HIn.
-              destruct HIn as [HIn HnIn]. rewrite Heq in HnIn; rewrite Resources.diff_notin_spec in HnIn.
-              destruct HnIn as [HnIn | HIn'].
-              ** assert (r ∈ R1 \ R')%rs. { rewrite Resources.diff_spec; split; assumption. }
-                  apply HInW in H as [HInW1 HnInV]; intro c; apply HnInV. 
-                  repeat rewrite RE.add_in_iff; repeat right.
-                  eapply RE.shift_in_spec in c as c'; rewrite Resource.shift_valid_refl in c'; eauto.
-                  eapply RE.valid_in_spec in c; eauto.
-              ** rewrite Hnew in HIn'. repeat rewrite Resources.add_spec in HIn'; 
-                  destruct HIn' as [Heq' | [Heq' | HIn']]; try (inversion HIn'); subst; 
-                  apply RE.Ext.new_key_notin_spec; lia.
-        + replace 2 with (1 + 1) by lia. rewrite Cell.shift_unfold.
-          replace ((newᵣᵦ(V)) + 1) with (S (newᵣᵦ(V))) by lia. 
-
-          assert (RE.eq ([⧐ᵣᵦ (newᵣᵦ(V)) ≤ 1 + 1] V) ([⧐ᵣᵦ S (newᵣᵦ(V)) ≤ 1] [⧐ᵣᵦ (newᵣᵦ(V)) ≤ 1] V)).
-          { rewrite RE.shift_unfold; replace ((newᵣᵦ(V)) + 1) with (S (newᵣᵦ(V))) by lia; reflexivity. }
-          rewrite H.
-      
-          assert (RE.eq (⌈ (newᵣᵦ(V)) ⤆ [⧐ᵣₓ S (newᵣᵦ(V)) ≤ 1] [⧐ᵣₓ (newᵣᵦ(V)) ≤ 1] ⩽ i … ⩾ ⌉ᵣᵦ ([⧐ᵣᵦ S (newᵣᵦ(V)) ≤ 1] [⧐ᵣᵦ (newᵣᵦ(V)) ≤ 1] V))
-                              ([⧐ᵣᵦ S (newᵣᵦ(V)) ≤ 1] (⌈ (newᵣᵦ(V)) ⤆ [⧐ᵣₓ (newᵣᵦ(V)) ≤ 1] ⩽ i … ⩾ ⌉ᵣᵦ ([⧐ᵣᵦ (newᵣᵦ(V)) ≤ 1] V)))).
-          { 
-            rewrite RE.shift_add_notin_spec.
-            - replace ([⧐ᵣ S (newᵣᵦ(V)) ≤ 1] (newᵣᵦ(V))) with (newᵣᵦ(V)); try reflexivity.
-              rewrite Resource.shift_valid_refl; auto; unfold Resource.valid; lia.
-            - apply RE.shift_new_notin_spec; lia.
-          }
-
-          rewrite H0; clear H H0.
-          eapply (itfT_init 
-                    (⌈ newᵣᵪ( Re) ⤆ (<[ 𝟙 ]>, τ) ⌉ᵣᵪ Re)
-                    (⌈ S (newᵣᵪ( Re)) ⤆ (τ, <[ 𝟙 ]>) ⌉ᵣᵪ (⌈ newᵣᵪ( Re) ⤆ (<[ 𝟙 ]>, τ) ⌉ᵣᵪ Re))
-                    (⌈ newᵣᵦ( V) ⤆ [⧐ᵣₓ newᵣᵦ( V) ≤ 1] ⩽ i … ⩾ ⌉ᵣᵦ ([⧐ᵣᵦ newᵣᵦ( V) ≤ 1] V))
-                    (⌈ S (newᵣᵦ( V)) ⤆ ⩽ unit … ⩾ ⌉ᵣᵦ ([⧐ᵣᵦ S (newᵣᵦ( V)) ≤ 1] ⌈ newᵣᵦ( V) ⤆ [⧐ᵣₓ newᵣᵦ( V) ≤ 1] ⩽ i … ⩾ ⌉ᵣᵦ ([⧐ᵣᵦ newᵣᵦ( V) ≤ 1] V)))
-                    τ <[𝟙]> <[unit]>); eauto; try now constructor.
-          ++ eapply (itfT_init Re (⌈ newᵣᵪ( Re) ⤆ (<[ 𝟙 ]>, τ) ⌉ᵣᵪ Re)
-                                  V (⌈ newᵣᵦ( V) ⤆ [⧐ᵣₓ newᵣᵦ( V) ≤ 1] ⩽ i … ⩾ ⌉ᵣᵦ ([⧐ᵣᵦ newᵣᵦ( V) ≤ 1] V))
-                                  <[𝟙]> τ); eauto; try constructor.
-          ++ rewrite RC.Ext.new_key_add_spec_1; auto.
-              * apply well_typed_implies_valid in Hwi; auto.
-                destruct Hwi; apply Typ.valid_weakening with (k := newᵣᵪ( Re)); auto.
-              * apply RC.Ext.new_key_notin_spec; auto.
-          ++ unfold RC.Add;
-            rewrite RC.Ext.new_key_add_spec_1; auto; try reflexivity.
-            apply RC.Ext.new_key_notin_spec; auto.
-          ++ unfold RE.Add; 
-            rewrite RE.Ext.new_key_add_spec_1; auto; try reflexivity.
-            * apply RE.shift_new_notin_spec; lia.
-            * rewrite RE.shift_new_spec; auto.
-        + rewrite Heqnk'. apply RE.halts_add_spec; split.
-          ++ simpl. exists <[unit]>. split; auto.
-          ++ apply RE.halts_add_spec; split.
-             * simpl; exists <[[⧐ₜₘ {newᵣᵦ( V)} ≤ 2] i]>; split; auto.
-               now apply Term.shift_value_iff.
-             * replace (S (S (newᵣᵦ(V)))) with (newᵣᵦ(V) + 2) by lia.
-               unfold RE.halts; intros r' v' Hfi. 
-               assert (r' ∈ᵣᵦ [⧐ᵣᵦ newᵣᵦ(V) ≤ 2] V). { exists v'; now apply RE.find_2. }
-               apply RE.shift_in_e_spec in H as H'; destruct H'; subst.
-               apply RE.shift_find_e_spec in Hfi as H'; destruct H'; subst.
-               apply RE.shift_find_spec in Hfi; apply HltV in Hfi.
-               destruct x0; simpl in *; destruct Hfi as [λ' [HmeT Hvλ]];
-               exists <[ [⧐ₜₘ{newᵣᵦ( V)} ≤ 2] λ' ]>; split; try (now apply Term.shift_value_iff);
-               apply multi_evaluate_valid_weakening with (k' := newᵣᵪ( Re) + 2) in HmeT; try lia; rewrite <- Hnew in *;
-               replace (newᵣᵪ( Re) + 2 - newᵣᵪ( Re)) with 2 in HmeT; try lia; auto.
-        + rewrite <- Hnew ; rewrite RC.new_key_wh_spec. 
-          replace (S (S (newᵣᵪ(Re)))) with (newᵣᵪ(Re) + 2) by lia.
-          destruct Hltst as [st'' [HmeT Hvlst'']]; exists <[[⧐ₜₘ {newᵣᵦ( V)} ≤ 2] st'']>; split.
-          ++ rewrite <- Hnew. apply multi_evaluate_valid_weakening with (k' := newᵣᵪ( Re) + 2) in HmeT; try lia.
-             replace (newᵣᵪ( Re) + 2 - newᵣᵪ( Re)) with 2 in HmeT; try lia; auto.
-          ++ now apply Term.shift_value_iff.
-    -- apply RC.Submap_add_spec_1.
-        + apply RC.Ext.new_key_notin_spec; rewrite RC.Ext.new_key_add_spec_1;
-          auto. apply RC.Ext.new_key_notin_spec; lia.
-        + apply RC.Submap_add_spec_1.
-          ++ apply RC.Ext.new_key_notin_spec; lia.
-          ++ apply RC.Submap_refl.
-Admitted.
+    apply evaluate_preserves_typing with (t' := t1) in Hwt as Hwt1; auto.
+    eapply IHk in HieT as IH; eauto; clear IHk.
+    destruct IH as [V' [tv' [t1' [HfT [Hlt1' [Hltv' HltV']]]]]].
+    exists V'; exists tv'; exists t1'; split; auto; eapply fT_eT; eauto.
+Qed.
 
 (** *** Proof of Resource safety
 
   **** Hypothesis
 
   Knowing the term sf is well typed (1), the stream term is also well typed (2),
-  there is a transition using the two previous terms (3) and each term in the
+   using the two previous terms (3) and each term in the
   environment is well typed to a type findable in the context if they are
-  the same resource name that mapped them (4);
+  the same resource name that mapped them (3);
 
   **** Results
 
-  We can state that:
+  There is a transition such that :
   - each interaction with resources is done with values never used before (5);
   - we can found a context and a resource set such as :
     - all resources that are not in the set R have the same state before and after the functional transition (6);
@@ -1940,248 +530,22 @@ Admitted.
 
 *)
 Theorem safety_resources_interaction :
-  forall (Re : ℜ) (V V' : 𝓥) (W : 𝐖) (sv sv' sf sf' : Λ) (τ τ' : Τ) (R : resources),
+  forall (Re : ℜ) (V V' : 𝓥) (tv tv' t t' : Λ) (τ τ' : Τ) (R : resources),
 
-    (* (1) *) ∅ᵥᵪ ⋅ Re ⊫ sf ∈ (τ ⟿ τ' ∣ R) ->
-    (* (2) *) ∅ᵥᵪ ⋅ Re ⊫ sv ∈ τ -> 
-    (* (3) *) ⪡ V ; sv ; sf ⪢ ⭆ ⪡ V' ; sv' ; sf' ; W ⪢ -> 
-    (* (4) *) Instᵣₜ(Re,V) ->
+    (* (1) *) ∅ᵥᵪ ⋅ Re ⊫ t ∈ (τ ⟿ τ' ∣ R) ->
+    (* (2) *) ∅ᵥᵪ ⋅ Re ⊫ tv ∈ τ -> 
+    (* (3) *) Instᵣₜ(Re,V) ->
 
 
-    (* (5) *) (forall (r : resource), (r ∈ R)%rs -> RE.unused r V) /\
+    (* (5) *) (forall (r : resource), (r ∈ R)%rs -> RE.unused r V) ->
 
     exists (Re' : ℜ) (R' : resources),
 
       (* (6) *) (forall (r : resource), (r ∉ R')%rs /\ (r ∈ᵣᵦ V) -> 
-                    ([⧐ᵣᵦ (newᵣᵦ(V)) ≤ ((newᵣᵦ(V')) - (newᵣᵦ(V)))] V) ⌊r⌋ᵣᵦ = V' ⌊r⌋ᵣᵦ) /\
+                    V ⌊r⌋ᵣᵦ = V' ⌊r⌋ᵣᵦ) /\
       (* (7) *) (forall (r : resource), (r ∈ R')%rs -> RE.used r V')
 .
 Proof.
-  intros Re V V' W sv sv' sf sf' τ2 τ2' R Hinst Hwt Hwst HfT.
-  eapply functional_preserves_typing in HfT; eauto.
-  destruct HfT as [Hunsd [Hlcl [Re' [R' [HSubRe  [HSubR' [Hinst' [_ [Hlcl1 [Husd [Hwsv' Hwsf']]]]]]]]]]].
-  split; auto; exists Re'; exists R'; split; auto.
-  intros r [HnIn HInV]; destruct (Resources.In_dec r R).
-  - apply HSubR' in i; contradiction.
-  - apply Hlcl; split; assumption.
-Qed.
+  intros. 
 
-(* begin hide *)
-(*
-(** ** Progress *)
-Section progress.
-
-
-  Theorem experiment_1 : 
-    forall (Re : ℜ) (V : 𝓥) (sv sf : Λ) (τ τ' : Τ) (R : resources),
-
-      value(sf) -> 
-      halts (newᵣᵪ(Re)) sv ->
-      halts_V V ->
-      (forall r, (r ∈ R)%rs -> RE.unused r V) ->
-      
-      Instᵣₜ(Re,V) ->
-      
-      ∅ᵥᵪ ⋅ Re ⊫ sf ∈ (τ ⟿ τ' ∣ R) -> 
-      ∅ᵥᵪ ⋅ Re ⊫ sv ∈ τ ->
-
-      exists (V' : 𝓥) (W : 𝐖) (sv' sf' : Λ), 
-        ⪡ V ; sv ; sf ⪢ ⭆ ⪡ V' ; sv' ; sf' ; W ⪢ /\
-        (halts (newᵣᵦ(V')) sv') /\
-        halts_V V'.
-  Proof.
-    intros. revert V sv H H0 H1 H2 H3 H5; dependent induction H4; intros;
-    try now inversion H.
-
-    - inversion H; clear H; subst. 
-      exists V;
-      exists ∅ₛₖ;
-      exists <[t sv]>; 
-      exists <[arr(t)]>; 
-      repeat split; auto.
-      -- now repeat constructor.
-      -- (* Définir une props pour t sv *) admit.
-    - inversion H0; subst; clear H0.
-      destruct H1 as [sv' [HmeT Hvsv']].
-      apply instantiation_valid in H5 as HvRe; destruct HvRe as [HvRe _].
-      apply multi_preserves_typing with (t' := sv') in H6; auto.
-      destruct sv'; inversion H6; inversion Hvsv'; subst.
-
-      eapply IHwell_typed in H11; eauto.
-      -- destruct H11 as [V' [W [sv' [sf' [HfT [Hltsv' HltV']]]]]].
-
-          exists V';
-          exists W;
-          exists <[⟨sv',[⧐ₜₘ {newᵣᵦ(V)} ≤ {(newᵣᵦ(V')) - (newᵣᵦ(V))}] sv'2⟩]>;
-          exists <[first(τ0 :sf')]>.
-          repeat split; auto.
-          + eapply fT_first; eauto.
-            apply instantiation_new in H5; now rewrite <- H5.
-          + destruct Hltsv' as [sv'' [HmeT' Hvsv'']].
-            exists <[⟨sv'', [⧐ₜₘ{newᵣᵦ(V)} ≤ {newᵣᵦ(V') - newᵣᵦ(V)}] sv'2⟩]>; split.
-            ++ now apply multi_pair1.
-            ++ constructor; auto; now apply Term.shift_value_iff.
-      -- exists sv'1; split; auto; apply multi_refl.
-    (* wt_comp *)
-    - admit.
-    (* wt_rsf *)
-    - clear H0.  
-
-      assert (RE.unused r V). { apply H3; now apply Resources.singleton_spec. }
-      destruct H0 as [sv' HfV].
-      
-      assert (Hvr : newᵣᵪ(Re) ⊩ᵣ r). 
-      { 
-        apply instantiation_valid in H4; destruct H4.
-        eapply RC.valid_find_spec in H0 as [Hvr _]; eauto. 
-      }
-    
-      exists (⌈ r ⤆ ⩽ … sv ⩾ ⌉ᵣᵦ V); 
-      exists ∅ₛₖ; 
-      exists sv';
-      exists <[rsf[r]]>; repeat split.
-      -- repeat rewrite Resource.shift_valid_refl; auto; now constructor.
-      -- rewrite RE.Ext.new_key_add_spec_3.
-         + now apply H2 in HfV.
-         + apply RE.in_find; intro c; rewrite HfV in c; inversion c.
-      -- unfold halts_V; intros r' v HfV'; rewrite RE.add_o in HfV';
-         destruct (Resource.eq_dec r r'); subst; rewrite RE.Ext.new_key_add_spec_3;
-         try (apply RE.in_find; intro c; rewrite HfV in c; inversion c).
-         + inversion HfV'; subst; clear HfV'.
-           apply instantiation_new in H4 as Hnew; now rewrite <- Hnew.
-         + apply H2 in HfV'; auto.
-    (* wt_wh *)
-    - clear IHwell_typed1. fold VContext.empty in *. inversion H2; subst; clear H2.
-      eapply weakening_ℜ_1 with (Re' := ⌈ S k ⤆ (τ0, <[ 𝟙 ]>) ⌉ᵣᵪ (⌈ k ⤆ (<[ 𝟙 ]>, τ0) ⌉ᵣᵪ Re)) in H7.
-      -- replace (newᵣᵪ( ⌈ S k ⤆ (τ0, <[ 𝟙 ]>) ⌉ᵣᵪ (⌈ k ⤆ (<[ 𝟙 ]>, τ0) ⌉ᵣᵪ Re)) - newᵣᵪ(Re)) with 2 in H7.
-         + eapply IHwell_typed2 with (V := (⌈(S k) ⤆ ⩽ <[unit]> … ⩾ ⌉ᵣᵦ 
-         (⌈k ⤆ [⧐ᵣₓ k ≤ 2] ⩽ i … ⩾⌉ᵣᵦ  ([⧐ᵣᵦ k ≤ 2] V)))) in H7; eauto.
-  Admitted.
-
-  (*
-  Theorem progress_of_functional_value : 
-    forall (Re : ℜ) (V : 𝓥) (sv sf : Λ) (τ τ' : Τ) (R : resources),
-      halts (newᵣᵪ(Re)) sv ->
-      halts_V V ->
-      (Forall_arr (fun t => forall s, halts (newᵣᵪ(Re)) <[t s]>) sf) ->
-
-      value(sf) -> Instᵣₜ(Re,V) ->
-      ∅ᵥᵪ ⋅ Re ⊫ sf ∈ (τ ⟿ τ' ∣ R) -> 
-      ∅ᵥᵪ ⋅ Re ⊫ sv ∈ τ ->
-
-      (exists (V' : 𝓥) (W : 𝐖) (sv' sf' : Λ), 
-        ⪡ V ; sv ; sf ⪢ ⭆ ⪡ V' ; sv' ; sf' ; W ⪢ /\
-        (halts (newᵣᵦ(V')) sv') /\
-        halts_V V').
-  Proof.
-    intros Re V sv sf τ τ' R Hltsv HltV HltFarr Hvsf Hinst Hwsf Hwsv.
-    eapply progress_of_functional_value_gen with (Re' := Re) in Hwsv as IH; eauto.
-    - destruct IH as [V' [W [sv' [sf' [HfT [Hltsv' HltV']]]]]].
-      replace <[[⧐ₜₘ{newᵣᵪ( Re)} ≤ {newᵣᵪ( Re) - newᵣᵪ( Re)}] sf]> with sf in HfT.
-      -- exists V'; exists W; exists sv'; exists sf'; auto.
-      -- symmetry; apply Term.eq_leibniz; replace (newᵣᵪ(Re) - newᵣᵪ(Re)) with 0 by lia.
-         now rewrite Term.shift_refl.
-    - apply instantiation_valid in Hinst; destruct Hinst; assumption.
-    - apply RC.Submap_refl.
-  Qed.
-
-  Theorem progress_of_functional : 
-    forall (Re : ℜ) (V : 𝓥) (sv sf : Λ) (τ τ' : Τ) (R : resources),
-      halts (newᵣᵪ(Re)) sf ->
-      halts (newᵣᵪ(Re)) sv ->
-      halts_V V ->
-      (Forall_arr (fun t => forall s, halts (newᵣᵪ(Re)) <[t s]>) sf) ->
-
-      Instᵣₜ(Re,V) ->
-      ∅ᵥᵪ ⋅ Re ⊫ sf ∈ (τ ⟿ τ' ∣ R) -> 
-      ∅ᵥᵪ ⋅ Re ⊫ sv ∈ τ ->
-
-      (exists (V' : 𝓥) (W : 𝐖) (sv' sf' : Λ), 
-            ⪡ V ; sv ; sf ⪢ ⭆ ⪡ V' ; sv' ; sf' ; W ⪢ /\
-            (halts (newᵣᵦ(V')) sv') /\
-            halts_V V').
-  Proof. 
-    intros Re V sv sf τ τ' R Hltsf; revert V sv τ τ' R; destruct Hltsf as [sf' [HmeT Hvsf]].
-    apply multi_indexed in HmeT as [k HieT]; revert Re sf sf' HieT Hvsf; induction k;
-    intros Re sf sf' HieT Hvsf' V sv τ τ' R Hltsv HltV HltFarr Hinst Hwsf Hwsv.
-    (* sf is a value *)
-    - inversion HieT; subst; clear HieT;
-      eapply progress_of_functional_value; eauto.
-    (* sf can be reduced at least one time *)
-    - inversion HieT; subst.
-
-      (* clean *)
-      clear HieT; rename y into sf1; rename H0 into HeT; rename H2 into HieT;
-      move Re after IHk; move sf before Re; move sf' before sf; move sf1 before sf'.
-      move sv before sf1; move V before Re; move τ before sv; move τ' before τ;
-      move R before τ'.
-      (* clean *)
-
-      apply instantiation_valid in Hinst as Hv; destruct Hv as [HvRe _].
-      apply evaluate_preserves_typing with (t' := sf1) in Hwsf as Hwsf1; auto.
-      eapply IHk in HieT as IH; eauto.
-      -- apply instantiation_new in Hinst as Hnew; rewrite Hnew in HeT; clear Hnew.
-         destruct IH as [V' [W [sv' [sf1' [HfT [Hltsv' HltV']]]]]].
-         exists V'; exists W; exists sv'; exists sf1'; split; auto.
-         eapply fT_eT; eauto.
-      -- (* ForAll_arr have to be preserved by evaluation transition *) admit.
-  Admitted.
-  *)
-
-End progress.
-*)
-(* end hide *)
-
-(** *** Some corollaries *)
-
-Corollary functional_preserves_instantiation : 
-  forall (Re : ℜ) (V V' : 𝓥) (W : 𝐖) (sv sv' sf sf' : Λ) (τ τ' : Τ) (R : resources),  
-    Instᵣₜ(Re,V) ->
-    ∅ᵥᵪ ⋅ Re ⊫ sf ∈ (τ ⟿ τ' ∣ R) -> 
-    ∅ᵥᵪ ⋅ Re ⊫ sv ∈ τ -> 
-    ⪡ V ; sv ; sf ⪢ ⭆ ⪡ V' ; sv' ; sf' ; W ⪢ -> 
-
-    exists Re', Instᵣₜ(Re',V').
-Proof.
-  intros Re V V' W sv sv' sf sf' τ2 τ2' R Hinst Hwt Hwst HfT.
-  eapply functional_preserves_typing in HfT; eauto.
-  destruct HfT as [_ [_ [Re' [_ [_  [_ [Hinst' [_ [_ [_ _]]]]]]]]]];
-  now exists Re'.
-Qed.
-
-
-Corollary functional_preserves_stream_typing : 
-  forall (Re : ℜ) (V V' : 𝓥) (W : 𝐖) (sv sv' sf sf' : Λ) (τ τ' : Τ) (R : resources),  
-    Instᵣₜ(Re,V) ->
-    ∅ᵥᵪ ⋅ Re ⊫ sf ∈ (τ ⟿ τ' ∣ R) -> 
-    ∅ᵥᵪ ⋅ Re ⊫ sv ∈ τ -> 
-    ⪡ V ; sv ; sf ⪢ ⭆ ⪡ V' ; sv' ; sf' ; W ⪢ -> 
-
-    exists Re', ∅ᵥᵪ ⋅ Re' ⊫ sv' ∈ τ'.
-Proof.
-  intros Re V V' W sv sv' sf sf' τ2 τ2' R Hinst Hwt Hwst HfT.
-  eapply functional_preserves_typing in HfT; eauto.
-  destruct HfT as [_ [_ [Re' [_ [_ [_  [_ [Hinst' [_ [_ [Hwsv' _]]]]]]]]]]];
-  now exists Re'.
-Qed.
-
-
-Corollary functional_preserves_typing_1 : 
-  forall (Re : ℜ) (V V' : 𝓥) (W : 𝐖) (sv sv' sf sf' : Λ) (τ τ' : Τ) (R : resources),
-
-    Instᵣₜ(Re,V) ->
-    ∅ᵥᵪ ⋅ Re ⊫ sf ∈ (τ ⟿ τ' ∣ R) ->
-    ∅ᵥᵪ ⋅ Re ⊫ sv ∈ τ -> 
-    ⪡ V ; sv ; sf ⪢ ⭆ ⪡ V' ; sv' ; sf' ; W ⪢ -> 
-
-    exists (Re' : ℜ) (R' : resources), 
-      Re ⊆ᵣᵪ Re' /\  (R ⊆ R')%rs /\ Instᵣₜ(Re',V') /\ 
-      ∅ᵥᵪ ⋅ Re' ⊫ sv' ∈ τ' /\
-      ∅ᵥᵪ ⋅ Re' ⊫ sf' ∈ (τ ⟿ τ' ∣ R').
-Proof.
-  intros Re V V' W sv sv' sf sf' τ2 τ2' R Hinst Hwt Hwst HfT.
-  eapply functional_preserves_typing in HfT; eauto.
-  destruct HfT as [_ [_ [Re' [R' [HSubRe  [HSubR' [Hinst' [_ [_ [_ [Hwsv' Hwsf']]]]]]]]]]];
-  exists Re'; now exists R'.
-Qed.
-*)
+ Admitted.
