theories/Temporal.v
@@ -1,3 +1,4 @@
+(*
 From Coq Require Import Lists.Streams micromega.Lia Relations.Relation_Definitions 
                         Classes.RelationClasses Relations.Relation_Operators.
 Require Import Resource Resources Term Typ Var Substitution 
@@ -95,3 +96,4 @@ Proof.
   apply initialization_unused in H as H'; destruct x; inversion H'.
   exists λ. now rewrite H2.
 Qed. 
+*)
